Tealeaves/Examples/SystemF/Rewriting.v
@@ -1,5 +1,7 @@
 From Tealeaves Require Export
-  Examples.SystemF.Syntax.
+  Examples.SystemF.Syntax
+  Simplification.Tests.Support
+  Simplification.MBinddt.
 
 Import Subset.Notations.
 Import Monoid.Notations.
@@ -7,6 +9,8 @@ Import Monoid.Notations.
 
 #[local] Arguments mbinddt {ix} {W}%type_scope {T} U%function_scope
   {MBind} {F}%function_scope {H H0 H1 A B} _ _.
+
+Ltac normalize := change (@K I2) with K2 in *.
 
 (** * Miscellaneous lemmas *)
 (******************************************************************************)
@@ -28,51 +32,6 @@ Qed.
 
 (** * Simplification support *)
 (******************************************************************************)
-
-(** Copied *)
-
-
-(** ** Monoid-related *)
-
-Ltac simplify_to_monoid :=
-  unfold_ops @Pure_const @Mult_const; simpl_monoid.
-
-Ltac extract_preincr :=
-    match goal with
-      |- context[((?f ∘ extract) ⦿ ?w)] =>
-        rewrite extract_preincr2
-    end.
-
-(** ** tolist/in-related *)
-Ltac tolist_to_binddt :=
-  rewrite tolist_to_traverse1, traverse_to_binddt.
-
-(*
-Search "to_foldMap".
-About element_to_foldMap_list1.
-Ltac in_to_binddt :=
-  rewrite in_to_foldMap, foldMap_to_traverse1, traverse_to_binddt.
-*)
-
-(** ** const/applicative/map related *)
-Lemma pure_const_rw: forall {A} {a:A} {M} {unit:Monoid_unit M},
-    pure (F := const M) (Pure := @Pure_const _ unit) a = Ƶ.
-  reflexivity.
-Qed.
-
-Lemma ap_const_rw: forall {M} `{Monoid_op M} {A B} (x: const M (A -> B)) (y: const M A),
-    ap (const M) x y = (x ● y).
-  reflexivity.
-Qed.
-
-Lemma map_const_rw: forall A B (f: A -> B) X,
-    map (F := const X) f = @id X.
-Proof.
-  reflexivity.
-Qed.
-
-(** /Copied *)
-
 Lemma mextract_preincr2 :
   forall `{ix: Index} {W : Type} {op : Monoid_op W}
     {A: Type} {B : K -> Type} (f: forall k, A -> B k) (w : W),
@@ -87,6 +46,11 @@ Qed.
 Create HintDb sysf_rw.
 Tactic Notation "simpl_F" := autorewrite with sysf_rw.
 
+(*
+#[export] Hint Rewrite @mbinddt_term_rw1 @mbinddt_term_rw2 @mbinddt_term_rw3 @mbinddt_term_rw4 @mbinddt_term_rw5 : sysf_rw.
+#[export] Hint Rewrite @mbinddt_type_rw1 @mbinddt_type_rw2 @mbinddt_type_rw3 @mbinddt_type_rw4 : sysf_rw.
+ *)
+
 Section rw_mbinddt.
 
   Context
@@ -96,30 +60,49 @@ Section rw_mbinddt.
 
   Lemma mbinddt_type_rw1 : forall c,
       mbinddt typ f (ty_c c) = pure (ty_c c).
-  Proof. reflexivity. Qed.
+  Proof.
+    intros.
+    cbn_mbinddt.
+    conclude.
+  Qed.
 
   Lemma mbinddt_type_rw2 : forall (a : A),
-      mbinddt typ f (ty_v a) = f KType (nil, a).
-  Proof. reflexivity. Qed.
+      mbinddt typ f (ty_v a) = f ktyp (nil, a).
+  Proof.
+    intros.
+    cbn_mbinddt.
+    normalize.
+    conclude.
+  Qed.
 
   Lemma mbinddt_type_rw3 : forall (t1 t2 : typ A),
       mbinddt typ f (ty_ar t1 t2) =
         pure ty_ar <⋆> mbinddt typ f t1 <⋆> mbinddt typ f t2.
-  Proof. reflexivity. Qed.
+  Proof.
+    intros.
+    cbn_mbinddt.
+    normalize.
+    conclude.
+  Qed.
 
   Lemma mbinddt_type_rw4 : forall (body : typ A),
       mbinddt typ f (ty_univ body) =
-        pure ty_univ <⋆> mbinddt typ (f ◻ const (incr [KType])) body.
-  Proof. reflexivity. Qed.
+        pure ty_univ <⋆> mbinddt typ (f ◻ allK (incr [ktyp])) body.
+  Proof.
+    intros.
+    cbn_mbinddt.
+    normalize.
+    conclude.
+    reflexivity. Qed.
 
   Lemma mbinddt_term_rw1 : forall (a : A),
-      mbinddt term f (tm_var a) = f KTerm (nil, a).
+      mbinddt term f (tm_var a) = f ktrm (nil, a).
   Proof. reflexivity. Qed.
 
   Lemma mbinddt_term_rw2 : forall (τ : typ A) (t : term A),
       mbinddt term f (tm_abs τ t) =
         pure tm_abs <⋆> (mbinddt typ f τ) <⋆>
-          (mbinddt term (f ◻ const (incr [KTerm])) t).
+          (mbinddt term (f ◻ const (incr [ktrm])) t).
   Proof. reflexivity. Qed.
 
   Lemma mbinddt_term_rw3 : forall (t1 t2 : term A),
@@ -129,7 +112,7 @@ Section rw_mbinddt.
 
   Lemma mbinddt_term_rw4 : forall (t : term A),
       mbinddt term f (tm_tab t) =
-        pure tm_tab <⋆> (mbinddt term (fun k => f k ∘ incr [KType]) t).
+        pure tm_tab <⋆> (mbinddt term (fun k => f k ∘ incr [ktyp]) t).
   Proof. reflexivity. Qed.
 
   Lemma mbinddt_term_rw5 : forall (t: term A) (τ : typ A),
@@ -139,8 +122,6 @@ Section rw_mbinddt.
 
 End rw_mbinddt.
 
-#[export] Hint Rewrite @mbinddt_term_rw1 @mbinddt_term_rw2 @mbinddt_term_rw3 @mbinddt_term_rw4 @mbinddt_term_rw5 : sysf_rw.
-#[export] Hint Rewrite @mbinddt_type_rw1 @mbinddt_type_rw2 @mbinddt_type_rw3 @mbinddt_type_rw4 : sysf_rw.
 
 Ltac simplify :=
   match goal with
@@ -155,465 +136,207 @@ Ltac simplify :=
             | rewrite mbinddt_term_rw3
             | rewrite mbinddt_term_rw4
             | rewrite mbinddt_term_rw5 ]
-  | |- context[(?f ∘ extract) ⦿ ?w] =>
-      rewrite extract_preincr2
-  | |- context[(?f ∘ extract) (?w, ?a)] =>
-      change ((f ∘ extract) (w, a)) with
-      ((f ∘ (extract ∘ pair w)) a);
-      rewrite extract_pair
-  | |- context [id ∘ ?f] =>
-      idtac "id ∘ f";
-      change (id ∘ f) with f
-  | |- context [?f ∘ id] =>
-      idtac "f ∘ id";
-      change (f ∘ id) with f
-  | |- context [pure (F := const ?W) ?x] =>
-      idtac "pure_const";
-      rewrite pure_const_rw
-  | |- context[(ap (const ?W) ?x ?y)] =>
-      idtac "ap_const";
-      rewrite ap_const_rw
-  | |- context[pure (F := fun A => A) ?x] =>
-      idtac "pure_I";
-      change (pure (F := fun A => A) x) with x
-  | |- context[(ap (fun A => A) ?x ?y)] =>
-      idtac "ap_I";
-      change (ap (fun A => A) x y) with (x y)
-  | |- context[Ƶ ● ?m] =>
-      idtac "monoid_id_r";
-      rewrite (monoid_id_r m)
-  | |- context[?m ● Ƶ] =>
-      idtac "monoid_id_l";
-      rewrite (monoid_id_l m)
-  | |- context[map (F := const ?X) ?f] =>
-      idtac "map_const";
-      rewrite map_const_rw
-  | |- context[map (F := const ?X)] =>
-      (* this case works binders *)
-      idtac "map_const_alt";
-      change (map (F := const ?M) ?f ∘ ?g) with g
-(*
-  | |- context[free_loc (Fr ?x)] =>
-      rewrite free_loc_Fr
-  | |- context[free_loc (Bd ?b)] =>
-      rewrite free_loc_Bd
-  | |- context[?x ∈ [?y]] =>
-      rewrite in_list_one
-  | |- context[Forall_ctx ?P] =>
-      unfold Forall_ctx
-  | |- context[is_bound_or_free] =>
-      simplify_is_bound_or_free
- *)
   (* new stuff *)
   | |- context[(?f ◻ const extract) ◻ const (incr ?w)] =>
       rewrite mextract_preincr2
   end.
 
-(*
-(** * Rewriting operations on <<typ>> *)
-(******************************************************************************)
-
-(** ** Fundamental operations *)
-(******************************************************************************)
-
-(** *** <<mmapdt>> *)
-(******************************************************************************)
-Section rw_mmapdt_type.
-
-  Context
-    (A B : Type)
-    `{Applicative F}
-    (f : K -> list K * A -> F B).
-
-  Lemma rw_mmapdt_type1:
-    forall c, mmapdt typ F f (ty_c c) = pure (ty_c c).
-  Proof.
-    intros.
-    rewrite mmapdt_to_mbinddt.
-    simplify.
-    reflexivity.
-  Qed.
-
-  (* Why is this expressed with <⋆>? *)
-  Lemma rw_mmapdt_type2: forall (a: A), mmapdt typ F f (ty_v a) = pure ty_v <⋆> f KType (nil, a).
-  Proof.
-    intros.
-    rewrite mmapdt_to_mbinddt.
-    simplify.
-    rewrite <- map_to_ap.
-    reflexivity.
-  Qed.
-
-  Lemma rw_mmapdt_type3: forall (t1 t2: typ A),
-      mmapdt typ F f (ty_ar t1 t2) =
-        pure (ty_ar) <⋆> mmapdt typ F f t1 <⋆> mmapdt typ F f t2.
-  Proof.
-    intros.
-    rewrite mmapdt_to_mbinddt.
-    simplify.
-    reflexivity.
-  Qed.
-
-  Lemma rw_mmapdt_type4: forall (body: typ A),
-      mmapdt typ F f (ty_univ body) =
-        pure (ty_univ) <⋆> mmapdt typ F (fun k => f k ∘ incr [KType]) body.
-  Proof.
-    reflexivity.
-  Qed.
-
-End rw_mmapdt_type.
-
-(*
-#[export] Hint Rewrite @rw_mmapdt_type1 @rw_mmapdt_type2 @rw_mmapdt_type3 @rw_mmapdt_type4: sysf_rw.
-*)
-
-(** *** <<mbindd>> *)
-(******************************************************************************)
-Section rw_mbindd_type.
-
-  Context
-    (A B: Type)
-    (f: forall k, list K * A -> SystemF k B).
-
-  Lemma rw_mbindd_type1: forall c, mbindd typ f (ty_c c) = ty_c c.
-  Proof. reflexivity. Qed.
-
-  Lemma rw_mbindd_type2: forall (a: A), mbindd typ f (ty_v a) = f KType (nil, a).
-  Proof. reflexivity. Qed.
-
-  Lemma rw_mbindd_type3: forall (t1 t2: typ A), mbindd typ f (ty_ar t1 t2) = ty_ar (mbindd typ f t1) (mbindd typ f t2).
-  Proof. reflexivity. Qed.
-
-  Lemma rw_mbindd_type4: forall (body: typ A), mbindd typ f (ty_univ body) = ty_univ (mbindd typ (fun k => f k ∘ incr [KType]) body).
-  Proof. reflexivity. Qed.
-
-End rw_mbindd_type.
-
-#[export] Hint Rewrite @rw_mbindd_type1 @rw_mbindd_type2 @rw_mbindd_type3 @rw_mbindd_type4: sysf_rw.
-
-(** *** <<mbind>> *)
-(******************************************************************************)
-Section rw_mbind_type.
-
-  Context
-    (A B: Type)
-    (f: forall k, A -> SystemF k B).
-
-  Lemma rw_mbind_type1: forall c, mbind typ f (ty_c c) = ty_c c.
-  Proof. reflexivity. Qed.
-
-  Lemma rw_mbind_type2: forall (a: A), mbind typ f (ty_v a) = f KType a.
-  Proof. reflexivity. Qed.
-
-  Lemma rw_mbind_type3: forall (t1 t2: typ A), mbind typ f (ty_ar t1 t2) = ty_ar (mbind typ f t1) (mbind typ f t2).
-  Proof. reflexivity. Qed.
-
-  Lemma rw_mbind_type4: forall (body: typ A), mbind typ f (ty_univ body) = ty_univ (mbind typ f body).
-  Proof.
-    intros. unfold mbind. rewrite rw_mbindd_type4. repeat fequal. now ext k [w a].
-  Qed.
-
-End rw_mbind_type.
-
-#[export] Hint Rewrite @rw_mbind_type1 @rw_mbind_type2 @rw_mbind_type3 @rw_mbind_type4: sysf_rw.
-
-(** *** <<kbindd>> with <<KType>> *)
-(******************************************************************************)
-Section rw_kbindd_type.
-
-  Context
-    (A: Type)
-    (f: list K * A -> typ A).
-
-  Lemma rw_kbindd_KType_type1: forall c, kbindd typ KType f (ty_c c) = ty_c c.
-  Proof. reflexivity. Qed.
-
-  Lemma rw_kbindd_KType_type2: forall a, kbindd typ KType f (ty_v a) = f (nil, a).
-  Proof. reflexivity. Qed.
-
-  Lemma rw_kbindd_KType_type3: forall (t1 t2: typ A), kbindd typ KType f (ty_ar t1 t2) = ty_ar (kbindd typ KType f t1) (kbindd typ KType f t2).
-  Proof. reflexivity. Qed.
-
-  Lemma rw_kbindd_KType_type4: forall (body: typ A), kbindd typ KType f (ty_univ body) = ty_univ (kbindd typ KType (f ∘ incr [KType]) body).
-  Proof.
-    intros. unfold kbindd. simpl_F.
-    do 2 fequal. now ext j [w a].
-  Qed.
-
-End rw_kbindd_type.
-
-#[export] Hint Rewrite @rw_kbindd_KType_type1 @rw_kbindd_KType_type2 @rw_kbindd_KType_type3 @rw_kbindd_KType_type4: sysf_rw.
-
-(** *** <<kbindd>> with <<KTerm>> *)
-(******************************************************************************)
-Section rw_kbindd_type.
-
-  Context
-    (A: Type)
-    (f: list K * A -> term A).
-
-  Lemma rw_kbindd_KTerm_type1: forall c, kbindd typ KTerm f (ty_c c) = ty_c c.
-  Proof. reflexivity. Qed.
-
-  Lemma rw_kbindd_KTerm_type2: forall a, kbindd typ KTerm f (ty_v a) = ty_v a.
-  Proof. reflexivity. Qed.
-
-  Lemma rw_kbindd_KTerm_type3: forall (t1 t2: typ A), kbindd typ KTerm f (ty_ar t1 t2) = ty_ar (kbindd typ KTerm f t1) (kbindd typ KTerm f t2).
-  Proof. reflexivity. Qed.
-
-  Lemma rw_kbindd_KTerm_type4: forall (body: typ A), kbindd typ KTerm f (ty_univ body) = ty_univ (kbindd typ KTerm (f ∘ incr [KType]) body).
-  Proof.
-    intros. unfold kbindd. simpl_F.
-    do 2 fequal. now ext j [w a].
-  Qed.
-
-End rw_kbindd_type.
-
-#[export] Hint Rewrite @rw_kbindd_KTerm_type1 @rw_kbindd_KTerm_type2 @rw_kbindd_KTerm_type3 @rw_kbindd_KTerm_type4: sysf_rw.
-
-(** *** <<kbind>> with <<KType>> *)
-(******************************************************************************)
-Section rw_kbind_type.
-
-  Context
-    (A: Type)
-    (f: A -> typ A).
-
-  Lemma rw_kbind_KType_type1: forall c, kbind typ KType f (ty_c c) = ty_c c.
-  Proof. reflexivity. Qed.
-
-  Lemma rw_kbind_KType_type2: forall a, kbind typ KType f (ty_v a) = f a.
-  Proof. reflexivity. Qed.
-
-  Lemma rw_kbind_KType_type3: forall (t1 t2: typ A), kbind typ KType f (ty_ar t1 t2) = ty_ar (kbind typ KType f t1) (kbind typ KType f t2).
-  Proof. reflexivity. Qed.
-
-  Lemma rw_kbind_KType_type4: forall (body: typ A), kbind typ KType f (ty_univ body) = ty_univ (kbind typ KType f body).
-  Proof.
-    intros. unfold kbind. now simpl_F.
-  Qed.
-
-End rw_kbind_type.
-
-#[export] Hint Rewrite @rw_kbind_KType_type1 @rw_kbind_KType_type2 @rw_kbind_KType_type3 @rw_kbind_KType_type4: sysf_rw.
-
-(** *** <<kbind>> with <<KTerm>> *)
-(******************************************************************************)
-Section rw_kbind_type.
-
-  Context
-    (A: Type)
-    (f: A -> term A).
-
-  Lemma rw_kbind_KTerm_type1: forall c, kbind typ KTerm f (ty_c c) = ty_c c.
-  Proof. reflexivity. Qed.
-
-  Lemma rw_kbind_KTerm_type2: forall a, kbind typ KTerm f (ty_v a) = ty_v a.
-  Proof. reflexivity. Qed.
-
-  Lemma rw_kbind_KTerm_type3: forall (t1 t2: typ A), kbind typ KTerm f (ty_ar t1 t2) = ty_ar (kbind typ KTerm f t1) (kbind typ KTerm f t2).
-  Proof. reflexivity. Qed.
-
-  Lemma rw_kbind_KTerm_type4: forall (body: typ A), kbind typ KTerm f (ty_univ body) = ty_univ (kbind typ KTerm f body).
-  Proof.
-    intros. unfold kbind. now simpl_F.
-  Qed.
-
-End rw_kbind_type.
-
-#[export] Hint Rewrite @rw_kbind_KTerm_type1 @rw_kbind_KTerm_type2 @rw_kbind_KTerm_type3 @rw_kbind_KTerm_type4: sysf_rw.
-
-*)
-
 
 (** ** List and occurrence operations *)
 (******************************************************************************)
 
-(** *** <<tomlistd>> *)
+(** *** <<tolistmd>> *)
 (******************************************************************************)
-Section rw_tomlistd_type.
+Section rw_tolistmd_type.
 
   Context
     (A: Type).
 
-  Lemma rw_tomlistd_type1: forall c,
-      tomlistd (A:= A) typ (ty_c c) = nil.
+  Lemma rw_tolistmd_type1: forall c,
+      tolistmd (A:= A) typ (ty_c c) = nil.
   Proof.
     reflexivity.
   Qed.
 
-  Lemma rw_tomlistd_type2: forall (a: A),
-      tomlistd typ (ty_v a) = [ (nil, (KType, a)) ].
+  Lemma rw_tolistmd_type2: forall (a: A),
+      tolistmd typ (ty_v a) = [ (nil, (ktyp, a)) ].
   Proof.
     reflexivity.
   Qed.
 
-  Lemma rw_tomlistd_type3: forall (t1 t2: typ A),
-      tomlistd typ (ty_ar t1 t2) = tomlistd typ t1 ++ tomlistd typ t2.
+  Lemma rw_tolistmd_type3: forall (t1 t2: typ A),
+      tolistmd typ (ty_ar t1 t2) = tolistmd typ t1 ++ tolistmd typ t2.
   Proof.
     reflexivity.
   Qed.
 
   (* TODO automate and generalize this proof *)
-  Lemma rw_tomlistd_type4: forall (body: typ A),
-      tomlistd typ (ty_univ body) = map (F:= list) (incr [KType]) (tomlistd typ body).
+  Lemma rw_tolistmd_type4: forall (body: typ A),
+      tolistmd typ (ty_univ body) = map (F:= list) (incr [ktyp]) (tolistmd typ body).
   Proof.
     intros.
-    unfold tomlistd, tomlistd_gen.
+    unfold tolistmd, tolistmd_gen.
     rewrite mmapdt_to_mbinddt.
     simplify.
     simplify.
     simplify.
     simplify.
     compose near body on right.
+    rewrite vec_compose_assoc.
     rewrite (dtp_mbinddt_morphism
-               (list (@K I2)) SystemF (const (list _))).
+               (list (@K I2))
+               SystemF
+               typ
                (const (list _))
-               (ϕ := (fun k => map (A := list K2 * (@K I2 * A))
-                             (F:= list) (Map := Map_list) (incr [KType])))).
+               (const (list _))
+               (ϕ := (fun k => map
+                              (A := list K2 * (@K I2 * A))
+                              (F := list)
+                              (Map := Map_list)
+                              (incr [ktyp])))).
     fequal. now ext k [w a].
   Qed.
 
-End rw_tomlistd_type.
+End rw_tolistmd_type.
 
-#[export] Hint Rewrite @rw_tomlistd_type1 @rw_tomlistd_type2 @rw_tomlistd_type3 @rw_tomlistd_type4: sysf_rw.
+#[export] Hint Rewrite @rw_tolistmd_type1 @rw_tolistmd_type2 @rw_tolistmd_type3 @rw_tolistmd_type4: sysf_rw.
 
-(** *** <<toklistd>> with <<KType>> *)
+(** *** <<toklistd>> with <<ktyp>> *)
 (******************************************************************************)
-Section rw_toklistd_KType_type.
+Section rw_toklistd_ktyp_type.
 
   Context
     (A: Type).
 
-  Lemma rw_toklistd_KType_type1: forall c,
-      toklistd (A:= A) typ KType (ty_c c) = nil.
+  Lemma rw_toklistd_ktyp_type1: forall c,
+      toklistd (A:= A) typ ktyp (ty_c c) = nil.
   Proof.
     reflexivity.
   Qed.
 
-  Lemma rw_toklistd_KType_type2: forall (a: A),
-      toklistd typ KType (ty_v a) = [ (nil, a) ].
+  Lemma rw_toklistd_ktyp_type2: forall (a: A),
+      toklistd typ ktyp (ty_v a) = [ (nil, a) ].
   Proof.
     reflexivity.
   Qed.
 
-  Lemma rw_toklistd_KType_type3: forall (t1 t2: typ A),
-      toklistd typ KType (ty_ar t1 t2) =
-        toklistd typ KType t1 ++ toklistd typ KType t2.
+  Lemma rw_toklistd_ktyp_type3: forall (t1 t2: typ A),
+      toklistd typ ktyp (ty_ar t1 t2) =
+        toklistd typ ktyp t1 ++ toklistd typ ktyp t2.
   Proof.
     intros.
     unfold toklistd, compose.
-    rewrite rw_tomlistd_type3.
+    rewrite rw_tolistmd_type3.
     now autorewrite with tea_list.
   Qed.
 
-  Lemma rw_toklistd_KType_type4: forall (body: typ A), toklistd typ KType (ty_univ body) = map (F:= list) (incr [KType]) (toklistd typ KType body).
-  Proof. intros. unfold toklistd, compose. rewrite rw_tomlistd_type4. now rewrite filterk_incr. Qed.
+  Lemma rw_toklistd_ktyp_type4: forall (body: typ A), toklistd typ ktyp (ty_univ body) = map (F:= list) (incr [ktyp]) (toklistd typ ktyp body).
+  Proof. intros. unfold toklistd, compose. rewrite rw_tolistmd_type4. now rewrite filterk_incr. Qed.
 
-End rw_toklistd_KType_type.
+End rw_toklistd_ktyp_type.
 
-#[export] Hint Rewrite @rw_toklistd_KType_type1 @rw_toklistd_KType_type2 @rw_toklistd_KType_type3 @rw_toklistd_KType_type4: sysf_rw.
+#[export] Hint Rewrite @rw_toklistd_ktyp_type1 @rw_toklistd_ktyp_type2 @rw_toklistd_ktyp_type3 @rw_toklistd_ktyp_type4: sysf_rw.
 
-(** *** <<toklistd>> with <<KTerm>> *)
+(** *** <<toklistd>> with <<ktrm>> *)
 (******************************************************************************)
-Section rw_toklistd_KTerm_type.
+Section rw_toklistd_ktrm_type.
 
   Context
     (A: Type).
 
-  Lemma rw_toklistd_KTerm_type1: forall c, toklistd (A:= A) typ KTerm (ty_c c) = nil.
+  Lemma rw_toklistd_ktrm_type1: forall c, toklistd (A:= A) typ ktrm (ty_c c) = nil.
   Proof. reflexivity. Qed.
 
-  Lemma rw_toklistd_KTerm_type2: forall (a: A), toklistd typ KTerm (ty_v a) = nil.
+  Lemma rw_toklistd_ktrm_type2: forall (a: A), toklistd typ ktrm (ty_v a) = nil.
   Proof. reflexivity. Qed.
 
-  Lemma rw_toklistd_KTerm_type3: forall (t1 t2: typ A), toklistd typ KTerm (ty_ar t1 t2) = toklistd typ KTerm t1 ++ toklistd typ KTerm t2.
-  Proof. intros. unfold toklistd, compose. rewrite rw_tomlistd_type3. now autorewrite with tea_list. Qed.
+  Lemma rw_toklistd_ktrm_type3: forall (t1 t2: typ A), toklistd typ ktrm (ty_ar t1 t2) = toklistd typ ktrm t1 ++ toklistd typ ktrm t2.
+  Proof. intros. unfold toklistd, compose. rewrite rw_tolistmd_type3. now autorewrite with tea_list. Qed.
 
-  Lemma rw_toklistd_KTerm_type4: forall (body: typ A), toklistd typ KTerm (ty_univ body) = map (F:= list) (incr [KType]) (toklistd typ KTerm body).
-  Proof. intros. unfold toklistd, compose. rewrite rw_tomlistd_type4. now rewrite filterk_incr. Qed.
+  Lemma rw_toklistd_ktrm_type4: forall (body: typ A), toklistd typ ktrm (ty_univ body) = map (F:= list) (incr [ktyp]) (toklistd typ ktrm body).
+  Proof. intros. unfold toklistd, compose. rewrite rw_tolistmd_type4. now rewrite filterk_incr. Qed.
 
-End rw_toklistd_KTerm_type.
+End rw_toklistd_ktrm_type.
 
-#[export] Hint Rewrite @rw_toklistd_KTerm_type1 @rw_toklistd_KTerm_type2 @rw_toklistd_KTerm_type3 @rw_toklistd_KTerm_type4: sysf_rw.
+#[export] Hint Rewrite @rw_toklistd_ktrm_type1 @rw_toklistd_ktrm_type2 @rw_toklistd_ktrm_type3 @rw_toklistd_ktrm_type4: sysf_rw.
 
-(** *** <<tomlist>> *)
+(** *** <<tolistm>> *)
 (******************************************************************************)
-Section rw_tomlist_type.
+Section rw_tolistm_type.
 
   Context
     (A: Type).
 
-  Lemma rw_tomlist_type1: forall c, tomlist (A:= A) typ (ty_c c) = nil.
+  Lemma rw_tolistm_type1: forall c, tolistm (A:= A) typ (ty_c c) = nil.
   Proof. reflexivity. Qed.
 
-  Lemma rw_tomlist_type2: forall (a: A), tomlist typ (ty_v a) = [ (KType, a) ].
+  Lemma rw_tolistm_type2: forall (a: A), tolistm typ (ty_v a) = [ (ktyp, a) ].
   Proof. reflexivity. Qed.
 
-  Lemma rw_tomlist_type3: forall (t1 t2: typ A), tomlist typ (ty_ar t1 t2) = tomlist typ t1 ++ tomlist typ t2.
-  Proof. intros. unfold tomlist, compose. rewrite rw_tomlistd_type3. now autorewrite with tea_list. Qed.
+  Lemma rw_tolistm_type3: forall (t1 t2: typ A), tolistm typ (ty_ar t1 t2) = tolistm typ t1 ++ tolistm typ t2.
+  Proof. intros. unfold tolistm, compose. rewrite rw_tolistmd_type3. now autorewrite with tea_list. Qed.
 
-  Lemma rw_tomlist_type4: forall (body: typ A), tomlist typ (ty_univ body) = (tomlist typ body).
-  Proof. intros. unfold tomlist, compose. rewrite rw_tomlistd_type4.
-         compose near (tomlistd typ body) on left. rewrite (fun_map_map (F:= list)).
+  Lemma rw_tolistm_type4: forall (body: typ A), tolistm typ (ty_univ body) = (tolistm typ body).
+  Proof. intros. unfold tolistm, compose. rewrite rw_tolistmd_type4.
+         compose near (tolistmd typ body) on left. rewrite (fun_map_map (F:= list)).
          fequal. now ext [w a].
   Qed.
 
-End rw_tomlist_type.
+End rw_tolistm_type.
 
-#[export] Hint Rewrite @rw_tomlist_type1 @rw_tomlist_type2 @rw_tomlist_type3 @rw_tomlist_type4: sysf_rw.
+#[export] Hint Rewrite @rw_tolistm_type1 @rw_tolistm_type2 @rw_tolistm_type3 @rw_tolistm_type4: sysf_rw.
 
-(** *** <<toklist>> with <<KType>> *)
+(** *** <<toklist>> with <<ktyp>> *)
 (******************************************************************************)
-Section rw_toklist_KType_type.
+Section rw_toklist_ktyp_type.
 
   Context
     (A: Type).
 
-  Lemma rw_toklist_KType_type1: forall c, toklist (A:= A) typ KType (ty_c c) = nil.
+  Lemma rw_toklist_ktyp_type1: forall c, toklist (A:= A) typ ktyp (ty_c c) = nil.
   Proof. reflexivity. Qed.
 
-  Lemma rw_toklist_KType_type2: forall (a: A), toklist typ KType (ty_v a) = [ a ].
+  Lemma rw_toklist_ktyp_type2: forall (a: A), toklist typ ktyp (ty_v a) = [ a ].
   Proof. reflexivity. Qed.
 
-  Lemma rw_toklist_KType_type3: forall (t1 t2: typ A), toklist typ KType (ty_ar t1 t2) = toklist typ KType t1 ++ toklist typ KType t2.
-  Proof. intros. unfold toklist, compose. rewrite rw_toklistd_KType_type3. now autorewrite with tea_list. Qed.
+  Lemma rw_toklist_ktyp_type3: forall (t1 t2: typ A), toklist typ ktyp (ty_ar t1 t2) = toklist typ ktyp t1 ++ toklist typ ktyp t2.
+  Proof. intros. unfold toklist, compose. rewrite rw_toklistd_ktyp_type3. now autorewrite with tea_list. Qed.
 
-  Lemma rw_toklist_KType_type4: forall (body: typ A), toklist typ KType (ty_univ body) = (toklist typ KType body).
-  Proof. intros. unfold toklist, compose. rewrite rw_toklistd_KType_type4.
-         compose near (toklistd typ KType body) on left. rewrite (fun_map_map (F:= list)).
+  Lemma rw_toklist_ktyp_type4: forall (body: typ A), toklist typ ktyp (ty_univ body) = (toklist typ ktyp body).
+  Proof. intros. unfold toklist, compose. rewrite rw_toklistd_ktyp_type4.
+         compose near (toklistd typ ktyp body) on left. rewrite (fun_map_map (F:= list)).
          fequal. now ext [w a]. Qed.
 
-End rw_toklist_KType_type.
+End rw_toklist_ktyp_type.
 
-#[export] Hint Rewrite @rw_toklist_KType_type1 @rw_toklist_KType_type2 @rw_toklist_KType_type3 @rw_toklist_KType_type4: sysf_rw.
+#[export] Hint Rewrite @rw_toklist_ktyp_type1 @rw_toklist_ktyp_type2 @rw_toklist_ktyp_type3 @rw_toklist_ktyp_type4: sysf_rw.
 
-(** *** <<toklist>> with <<KTerm>> *)
+(** *** <<toklist>> with <<ktrm>> *)
 (******************************************************************************)
-Section rw_toklist_KTerm_type.
+Section rw_toklist_ktrm_type.
 
   Context
     (A: Type).
 
-  Lemma rw_toklist_KTerm_type1: forall c, toklist (A:= A) typ KTerm (ty_c c) = nil.
+  Lemma rw_toklist_ktrm_type1: forall c, toklist (A:= A) typ ktrm (ty_c c) = nil.
   Proof. reflexivity. Qed.
 
-  Lemma rw_toklist_KTerm_type2: forall (a: A), toklist typ KTerm (ty_v a) = nil.
+  Lemma rw_toklist_ktrm_type2: forall (a: A), toklist typ ktrm (ty_v a) = nil.
   Proof. reflexivity. Qed.
 
-  Lemma rw_toklist_KTerm_type3: forall (t1 t2: typ A), toklist typ KTerm (ty_ar t1 t2) = toklist typ KTerm t1 ++ toklist typ KTerm t2.
-  Proof. intros. unfold toklist, compose. rewrite rw_toklistd_KTerm_type3. now autorewrite with tea_list. Qed.
+  Lemma rw_toklist_ktrm_type3: forall (t1 t2: typ A), toklist typ ktrm (ty_ar t1 t2) = toklist typ ktrm t1 ++ toklist typ ktrm t2.
+  Proof. intros. unfold toklist, compose. rewrite rw_toklistd_ktrm_type3. now autorewrite with tea_list. Qed.
 
-  Lemma rw_toklist_KTerm_type4: forall (body: typ A), toklist typ KTerm (ty_univ body) = (toklist typ KTerm body).
-  Proof. intros. unfold toklist, compose. rewrite rw_toklistd_KTerm_type4.
-         compose near (toklistd typ KTerm body) on left. rewrite (fun_map_map (F:= list)).
+  Lemma rw_toklist_ktrm_type4: forall (body: typ A), toklist typ ktrm (ty_univ body) = (toklist typ ktrm body).
+  Proof. intros. unfold toklist, compose. rewrite rw_toklistd_ktrm_type4.
+         compose near (toklistd typ ktrm body) on left. rewrite (fun_map_map (F:= list)).
          fequal. now ext [w a]. Qed.
 
-End rw_toklist_KTerm_type.
+End rw_toklist_ktrm_type.
 
-#[export] Hint Rewrite @rw_toklist_KTerm_type1 @rw_toklist_KTerm_type2 @rw_toklist_KTerm_type3 @rw_toklist_KTerm_type4: sysf_rw.
+#[export] Hint Rewrite @rw_toklist_ktrm_type1 @rw_toklist_ktrm_type2 @rw_toklist_ktrm_type3 @rw_toklist_ktrm_type4: sysf_rw.
 
-Corollary rw_toklist_KTerm_type: forall A (τ: typ A), toklist typ KTerm τ = nil.
+Corollary rw_toklist_ktrm_type: forall A (τ: typ A), toklist typ ktrm τ = nil.
 Proof.
   intros. induction τ; autorewrite with sysf_rw.
   - trivial.
@@ -624,7 +347,7 @@ Qed.
 
 (** *** Variable occurrence with context *)
 (******************************************************************************)
-Section rw_tomsetd_type.
+Section rw_tosetmd_type.
 
   Context
     (A: Type)
@@ -633,14 +356,14 @@ Section rw_tomsetd_type.
   Implicit Types
            (w: list K) (a: A).
 
-  Lemma rw_tomsetd_type1: forall c w a, (w, (k, a)) ∈md (ty_c c) <-> False.
+  Lemma rw_tosetmd_type1: forall c w a, (w, (k, a)) ∈md (ty_c c) <-> False.
   Proof.
-    intros. unfold tomsetd, compose. autorewrite with sysf_rw. easy.
+    intros. unfold tosetmd, compose. autorewrite with sysf_rw. easy.
   Qed.
 
-  Lemma rw_tomsetd_type2: forall w a a', (w, (k, a)) ∈md (ty_v a') <-> w = nil /\ k = KType /\ a = a'.
+  Lemma rw_tosetmd_type2: forall w a a', (w, (k, a)) ∈md (ty_v a') <-> w = nil /\ k = ktyp /\ a = a'.
   Proof.
-    intros. unfold tomsetd, compose.
+    intros. unfold tosetmd, compose.
     autorewrite with sysf_rw.
     rewrite tosubset_list_one.
     split.
@@ -648,26 +371,26 @@ Section rw_tomsetd_type.
     - firstorder. now subst.
   Qed.
 
-  Lemma rw_tomsetd_type3: forall w a (t1 t2: typ A), (w, (k, a)) ∈md ty_ar t1 t2 <-> ((w, (k, a)) ∈md t1 \/ (w, (k, a)) ∈md t2).
+  Lemma rw_tosetmd_type3: forall w a (t1 t2: typ A), (w, (k, a)) ∈md ty_ar t1 t2 <-> ((w, (k, a)) ∈md t1 \/ (w, (k, a)) ∈md t2).
   Proof.
-    intros. unfold tomsetd, compose.
+    intros. unfold tosetmd, compose.
     now autorewrite with sysf_rw tea_list tea_set.
   Qed.
 
-  Lemma rw_tomsetd_type4: forall w a (body: typ A), (w, (k, a)) ∈md (ty_univ body) <-> exists w', (w', (k, a)) ∈md body /\ w = (cons KType w').
+  Lemma rw_tosetmd_type4: forall w a (body: typ A), (w, (k, a)) ∈md (ty_univ body) <-> exists w', (w', (k, a)) ∈md body /\ w = (cons ktyp w').
   Proof.
-    intros. unfold tomsetd, compose. autorewrite with sysf_rw.
+    intros. unfold tosetmd, compose. autorewrite with sysf_rw.
     rewrite (tosubset_map_iff).
     splits.
     - intros [[w'' [j a']] [rest1 rest2]]. cbn in *. inverts rest2. eauto.
     - intros [w' rest]. exists (w', (k, a)). now inverts rest.
   Qed.
 
-End rw_tomsetd_type.
+End rw_tosetmd_type.
 
-#[export] Hint Rewrite @rw_tomsetd_type1 @rw_tomsetd_type2 @rw_tomsetd_type3 @rw_tomsetd_type4: sysf_rw.
+#[export] Hint Rewrite @rw_tosetmd_type1 @rw_tosetmd_type2 @rw_tosetmd_type3 @rw_tosetmd_type4: sysf_rw.
 
-Corollary rw_tomsetd_type_KTerm: forall w A a (τ: typ A), (w, (KTerm, a)) ∈md τ <-> False.
+Corollary rw_tosetmd_type_ktrm: forall w A a (τ: typ A), (w, (ktrm, a)) ∈md τ <-> False.
 Proof.
   intros. generalize dependent w.
   induction τ; intro w; autorewrite with sysf_rw; try easy.
@@ -678,7 +401,7 @@ Qed.
 
 (** *** Variable occurrence without context *)
 (******************************************************************************)
-Section rw_tomset_type.
+Section rw_tosetm_type.
 
   Context
     (A: Type)
@@ -686,123 +409,142 @@ Section rw_tomset_type.
 
   Implicit Types (a: A).
 
-  Lemma rw_tomset_type1: forall c a, (k, a) ∈m (ty_c c) <-> False.
-  Proof. intros. rewrite ind_iff_in. firstorder eauto. Qed.
+  Lemma rw_tosetm_type1: forall c a, (k, a) ∈m (ty_c c) <-> False.
+  Proof.
+    intros.
+    rewrite inmd_iff_in.
+    firstorder eauto.
+  Qed.
 
-  Lemma rw_tomset_type2: forall a a', (k, a) ∈m (ty_v a') <-> k = KType /\ a = a'.
-  Proof. intros. rewrite ind_iff_in. setoid_rewrite rw_tomsetd_type2. firstorder eauto.  Qed.
+  Lemma rw_tosetm_type2: forall a a', (k, a) ∈m (ty_v a') <-> k = ktyp /\ a = a'.
+  Proof.
+    intros.
+    rewrite inmd_iff_in.
+    setoid_rewrite rw_tosetmd_type2.
+    firstorder eauto.
+  Qed.
 
-  Lemma rw_tomset_type3: forall a (t1 t2: typ A), (k, a) ∈m ty_ar t1 t2 <-> (k, a) ∈m t1 \/ (k, a) ∈m t2.
-  Proof. intros. repeat rewrite ind_iff_in. setoid_rewrite rw_tomsetd_type3. firstorder eauto. Qed.
+  Lemma rw_tosetm_type3: forall a (t1 t2: typ A), (k, a) ∈m ty_ar t1 t2 <-> (k, a) ∈m t1 \/ (k, a) ∈m t2.
+  Proof.
+    intros.
+    repeat rewrite inmd_iff_in.
+    setoid_rewrite rw_tosetmd_type3.
+    firstorder eauto.
+  Qed.
 
-  Lemma rw_tomset_type4: forall a (body: typ A), (k, a) ∈m (ty_univ body) <-> (k, a) ∈m body.
-  Proof. intros. repeat rewrite ind_iff_in. setoid_rewrite rw_tomsetd_type4. firstorder eauto.  Qed.
+  Lemma rw_tosetm_type4: forall a (body: typ A), (k, a) ∈m (ty_univ body) <-> (k, a) ∈m body.
+  Proof.
+    intros.
+    repeat rewrite inmd_iff_in.
+    setoid_rewrite rw_tosetmd_type4.
+    firstorder eauto.
+  Qed.
 
-End rw_tomset_type.
+End rw_tosetm_type.
 
-#[export] Hint Rewrite @rw_tomset_type1 @rw_tomset_type2 @rw_tomset_type3 @rw_tomset_type4: sysf_rw.
+#[export] Hint Rewrite @rw_tosetm_type1 @rw_tosetm_type2 @rw_tosetm_type3 @rw_tosetm_type4: sysf_rw.
 
-(** ** <<free>> and <<freeset>> *)
+(** ** <<free>> and <<FV>> *)
 (******************************************************************************)
 
-(** *** <<free>> with <<KType>> *)
+(** *** <<free>> with <<ktyp>> *)
 (******************************************************************************)
-Section rw_free_KType_type.
+Section rw_free_ktyp_type.
 
-  Lemma rw_free_KType_type11: forall (x: atom), free typ KType (ty_v (Fr x)) = [x].
+  Lemma rw_free_ktyp_type11: forall (x: atom), free typ ktyp (ty_v (Fr x)) = [x].
   Proof.
     reflexivity.
   Qed.
 
-  Lemma rw_free_KType_type12: forall (n: nat), free typ KType (ty_v (Bd n)) = [].
+  Lemma rw_free_ktyp_type12: forall (n: nat), free typ ktyp (ty_v (Bd n)) = [].
   Proof.
     reflexivity.
   Qed.
 
-  Lemma rw_free_KType_type2: forall (c: base_typ), free typ KType (ty_c c) = [].
+  Lemma rw_free_ktyp_type2: forall (c: base_typ), free typ ktyp (ty_c c) = [].
   Proof.
     reflexivity.
   Qed.
 
-  Lemma rw_free_KType_type3: forall t1 t2, free typ KType (ty_ar t1 t2) = free typ KType t1 ++ free typ KType t2.
+  Lemma rw_free_ktyp_type3: forall t1 t2, free typ ktyp (ty_ar t1 t2) = free typ ktyp t1 ++ free typ ktyp t2.
   Proof.
     intros. unfold free. now autorewrite with sysf_rw tea_list.
   Qed.
 
-  Lemma rw_free_KType_type4: forall t, free typ KType (ty_univ t) = free typ KType t.
+  Lemma rw_free_ktyp_type4: forall t, free typ ktyp (ty_univ t) = free typ ktyp t.
   Proof.
     intros. unfold free. now autorewrite with sysf_rw tea_list.
   Qed.
 
-End rw_free_KType_type.
+End rw_free_ktyp_type.
 
-#[export] Hint Rewrite rw_free_KType_type11 rw_free_KType_type12 rw_free_KType_type2 rw_free_KType_type3 rw_free_KType_type4: sysf_rw.
+#[export] Hint Rewrite rw_free_ktyp_type11 rw_free_ktyp_type12 rw_free_ktyp_type2 rw_free_ktyp_type3 rw_free_ktyp_type4: sysf_rw.
 
-(** *** <<freeset>> with <<KType>> *)
+(** *** <<FV>> with <<ktyp>> *)
 (******************************************************************************)
-Section rw_freeset_KType_type.
+Section rw_fv_ktyp_type.
 
   #[local] Open Scope set_scope.
 
-  Lemma rw_freeset_KType_type11: forall (x: atom), freeset typ KType (ty_v (Fr x)) [=] {{ x }}.
+  Lemma rw_fv_ktyp_type11: forall (x: atom), FV typ ktyp (ty_v (Fr x)) [=] {{ x }}.
   Proof.
-    unfold freeset. intros. autorewrite with sysf_rw tea_rw_atoms. fsetdec.
+    unfold FV. intros. autorewrite with sysf_rw tea_rw_atoms. fsetdec.
   Qed.
 
-  Lemma rw_freeset_KType_type12: forall (n: nat), freeset typ KType (ty_v (Bd n)) [=] ∅.
-  Proof.
-    reflexivity.
-  Qed.
-
-  Lemma rw_freeset_KType_type2: forall (c: base_typ), freeset typ KType (ty_c c) [=] ∅.
+  Lemma rw_fv_ktyp_type12: forall (n: nat), FV typ ktyp (ty_v (Bd n)) [=] ∅.
   Proof.
     reflexivity.
   Qed.
 
-  Lemma rw_freeset_KType_type3: forall t1 t2, freeset typ KType (ty_ar t1 t2) [=] freeset typ KType t1 ∪ freeset typ KType t2.
+  Lemma rw_fv_ktyp_type2: forall (c: base_typ), FV typ ktyp (ty_c c) [=] ∅.
   Proof.
-    intros. unfold freeset. autorewrite with sysf_rw tea_rw_atoms. reflexivity.
+    reflexivity.
   Qed.
 
-  Lemma rw_freeset_KType_type4: forall t, freeset typ KType (ty_univ t) [=] freeset typ KType t.
+  Lemma rw_fv_ktyp_type3: forall t1 t2, FV typ ktyp (ty_ar t1 t2) [=] FV typ ktyp t1 ∪ FV typ ktyp t2.
   Proof.
-    intros. unfold freeset. autorewrite with sysf_rw tea_rw_atoms. reflexivity.
+    intros. unfold FV. autorewrite with sysf_rw tea_rw_atoms. reflexivity.
   Qed.
 
-End rw_freeset_KType_type.
+  Lemma rw_fv_ktyp_type4: forall t, FV typ ktyp (ty_univ t) [=] FV typ ktyp t.
+  Proof.
+    intros. unfold FV. autorewrite with sysf_rw tea_rw_atoms. reflexivity.
+  Qed.
 
-#[export] Hint Rewrite rw_freeset_KType_type11 rw_freeset_KType_type12 rw_freeset_KType_type2 rw_freeset_KType_type3 rw_freeset_KType_type4: sysf_rw.
+End rw_fv_ktyp_type.
 
-(** *** <<free>> with <<KTerm>> *)
+#[export] Hint Rewrite rw_fv_ktyp_type11 rw_fv_ktyp_type12 rw_fv_ktyp_type2 rw_fv_ktyp_type3 rw_fv_ktyp_type4: sysf_rw.
+
+(** *** <<free>> with <<ktrm>> *)
 (******************************************************************************)
-Section rw_free_KTerm_type.
+Section rw_free_ktrm_type.
 
-  Lemma rw_free_KTerm_type11: forall (x: atom), free typ KTerm (ty_v (Fr x)) = [].
+  Lemma rw_free_ktrm_type11: forall (x: atom), free typ ktrm (ty_v (Fr x)) = [].
   Proof.
     reflexivity.
   Qed.
 
-  Lemma rw_free_KTerm_type12: forall (n: nat), free typ KTerm (ty_v (Bd n)) = [].
+  Lemma rw_free_ktrm_type12: forall (n: nat), free typ ktrm (ty_v (Bd n)) = [].
   Proof.
     reflexivity.
   Qed.
 
-  Lemma rw_free_KTerm_type2: forall (c: base_typ), free typ KTerm (ty_c c) = [].
+  Lemma rw_free_ktrm_type2: forall (c: base_typ), free typ ktrm (ty_c c) = [].
   Proof.
     reflexivity.
   Qed.
 
-  Lemma rw_free_KTerm_type3: forall t1 t2, free typ KTerm (ty_ar t1 t2) = free typ KTerm t1 ++ free typ KTerm t2.
+  Lemma rw_free_ktrm_type3: forall t1 t2, free typ ktrm (ty_ar t1 t2) = free typ ktrm t1 ++ free typ ktrm t2.
   Proof. intros. unfold free. now autorewrite with sysf_rw tea_list. Qed.
 
-  Lemma rw_free_KTerm_type4: forall t, free typ KTerm (ty_univ t) = free typ KTerm t.
+  Lemma rw_free_ktrm_type4: forall t, free typ ktrm (ty_univ t) = free typ ktrm t.
   Proof. intros. unfold free. now autorewrite with sysf_rw tea_list. Qed.
 
-End rw_free_KTerm_type.
+End rw_free_ktrm_type.
 
-#[export] Hint Rewrite rw_free_KTerm_type11 rw_free_KTerm_type12 rw_free_KTerm_type2 rw_free_KTerm_type3 rw_free_KTerm_type4: sysf_rw.
+#[export] Hint Rewrite rw_free_ktrm_type11 rw_free_ktrm_type12 rw_free_ktrm_type2 rw_free_ktrm_type3 rw_free_ktrm_type4: sysf_rw.
 
-Corollary rw_free_KTerm_type: forall (τ: typ LN), free typ KTerm τ = [].
+Corollary rw_free_ktrm_type: forall (τ: typ LN), free typ ktrm τ = [].
 Proof.
   intros. induction τ; autorewrite with sysf_rw.
   - trivial.
@@ -811,41 +553,41 @@ Proof.
   - now rewrite IHτ.
 Qed.
 
-(** *** <<freeset>> with <<KTerm>> *)
+(** *** <<FV>> with <<ktrm>> *)
 (******************************************************************************)
-Section rw_freeset_KTerm_type.
+Section rw_fv_ktrm_type.
 
   #[local] Open Scope set_scope.
 
-  Lemma rw_freeset_KTerm_type11: forall (x: atom), freeset typ KTerm (ty_v (Fr x)) [=] ∅.
+  Lemma rw_fv_ktrm_type11: forall (x: atom), FV typ ktrm (ty_v (Fr x)) [=] ∅.
   Proof.
-    unfold freeset. intros. rewrite rw_free_KTerm_type11. autorewrite with tea_rw_atoms. fsetdec. Qed.
+    unfold FV. intros. rewrite rw_free_ktrm_type11. autorewrite with tea_rw_atoms. fsetdec. Qed.
 
-  Lemma rw_freeset_KTerm_type12: forall (n: nat), freeset typ KTerm (ty_v (Bd n)) [=] ∅.
-  Proof.
-    reflexivity.
-  Qed.
-
-  Lemma rw_freeset_KTerm_type2: forall (c: base_typ), freeset typ KTerm (ty_c c) [=] ∅.
+  Lemma rw_fv_ktrm_type12: forall (n: nat), FV typ ktrm (ty_v (Bd n)) [=] ∅.
   Proof.
     reflexivity.
   Qed.
 
-  Lemma rw_freeset_KTerm_type3: forall t1 t2, freeset typ KTerm (ty_ar t1 t2) [=] freeset typ KTerm t1 ∪ freeset typ KTerm t2.
+  Lemma rw_fv_ktrm_type2: forall (c: base_typ), FV typ ktrm (ty_c c) [=] ∅.
   Proof.
-    intros. unfold freeset. autorewrite with sysf_rw tea_rw_atoms. reflexivity.
+    reflexivity.
   Qed.
 
-  Lemma rw_freeset_KTerm_type4: forall t, freeset typ KTerm (ty_univ t) [=] freeset typ KTerm t.
+  Lemma rw_fv_ktrm_type3: forall t1 t2, FV typ ktrm (ty_ar t1 t2) [=] FV typ ktrm t1 ∪ FV typ ktrm t2.
   Proof.
-    intros. unfold freeset. autorewrite with sysf_rw tea_rw_atoms. reflexivity.
+    intros. unfold FV. autorewrite with sysf_rw tea_rw_atoms. reflexivity.
   Qed.
 
-End rw_freeset_KTerm_type.
+  Lemma rw_fv_ktrm_type4: forall t, FV typ ktrm (ty_univ t) [=] FV typ ktrm t.
+  Proof.
+    intros. unfold FV. autorewrite with sysf_rw tea_rw_atoms. reflexivity.
+  Qed.
 
-#[export] Hint Rewrite rw_freeset_KTerm_type11 rw_freeset_KTerm_type12 rw_freeset_KTerm_type2 rw_freeset_KTerm_type3 rw_freeset_KTerm_type4: sysf_rw.
+End rw_fv_ktrm_type.
 
-Corollary rw_freeset_KTerm_type: forall (τ: typ LN), (freeset typ KTerm τ [=] ∅)%set.
+#[export] Hint Rewrite rw_fv_ktrm_type11 rw_fv_ktrm_type12 rw_fv_ktrm_type2 rw_fv_ktrm_type3 rw_fv_ktrm_type4: sysf_rw.
+
+Corollary rw_fv_ktrm_type: forall (τ: typ LN), (FV typ ktrm τ [=] ∅)%set.
 Proof.
   intros. induction τ.
   - autorewrite with sysf_rw. fsetdec.
@@ -854,7 +596,7 @@ Proof.
   - autorewrite with sysf_rw. fsetdec.
 Qed.
 
-#[export] Hint Rewrite rw_freeset_KTerm_type: sysf_rw.
+#[export] Hint Rewrite rw_fv_ktrm_type: sysf_rw.
 
 (** ** Locally nameless operations *)
 (******************************************************************************)
@@ -866,37 +608,37 @@ Section rw_open_type.
   Context
     (u: typ LN).
 
-  Lemma rw_open_type1: forall c, open typ KType u (ty_c c) = ty_c c.
+  Lemma rw_open_type1: forall c, open typ ktyp u (ty_c c) = ty_c c.
   Proof. reflexivity. Qed.
 
-  Lemma rw_open_type2: forall (l: LN), open typ KType u (ty_v l) = open_loc KType u (nil, l).
+  Lemma rw_open_type2: forall (l: LN), open typ ktyp u (ty_v l) = open_loc ktyp u (nil, l).
   Proof. reflexivity. Qed.
 
-  Lemma rw_open_type3: forall (t1 t2: typ LN), open typ KType u (ty_ar t1 t2) = ty_ar (open typ KType u t1) (open typ KType u t2).
+  Lemma rw_open_type3: forall (t1 t2: typ LN), open typ ktyp u (ty_ar t1 t2) = ty_ar (open typ ktyp u t1) (open typ ktyp u t2).
   Proof. reflexivity. Qed.
 
 End rw_open_type.
 
 #[export] Hint Rewrite @rw_open_type1 @rw_open_type2 @rw_open_type3: sysf_rw.
 
-(** *** <<subst>> with <<KType>> *)
+(** *** <<subst>> with <<ktyp>> *)
 (******************************************************************************)
-Section rw_subst_KType_type.
+Section rw_subst_ktyp_type.
 
   Context
     (x: atom)
     (u: typ LN).
 
-  Lemma rw_subst_KType_type1: forall c, subst typ KType x u (ty_c c) = ty_c c.
+  Lemma rw_subst_ktyp_type1: forall c, subst typ ktyp x u (ty_c c) = ty_c c.
   Proof. reflexivity. Qed.
 
-  Lemma rw_subst_KType_type2: forall (l: LN), subst typ KType x u (ty_v l) = subst_loc KType x u l.
+  Lemma rw_subst_ktyp_type2: forall (l: LN), subst typ ktyp x u (ty_v l) = subst_loc ktyp x u l.
   Proof. reflexivity. Qed.
 
-  Lemma rw_subst_KType_type3: forall (t1 t2: typ LN), subst typ KType x u (ty_ar t1 t2) = ty_ar (subst typ KType x u t1) (subst typ KType x u t2).
+  Lemma rw_subst_ktyp_type3: forall (t1 t2: typ LN), subst typ ktyp x u (ty_ar t1 t2) = ty_ar (subst typ ktyp x u t1) (subst typ ktyp x u t2).
   Proof. reflexivity. Qed.
 
-  Lemma rw_subst_KType_type4: forall (t: typ LN), subst typ KType x u (ty_univ t) = ty_univ (subst typ KType x u t).
+  Lemma rw_subst_ktyp_type4: forall (t: typ LN), subst typ ktyp x u (ty_univ t) = ty_univ (subst typ ktyp x u t).
   Proof.
     intros.
     unfold subst.
@@ -910,28 +652,28 @@ Section rw_subst_KType_type.
     reflexivity.
   Qed.
 
-End rw_subst_KType_type.
+End rw_subst_ktyp_type.
 
-#[export] Hint Rewrite @rw_subst_KType_type1 @rw_subst_KType_type2 @rw_subst_KType_type3 @rw_subst_KType_type4: sysf_rw.
+#[export] Hint Rewrite @rw_subst_ktyp_type1 @rw_subst_ktyp_type2 @rw_subst_ktyp_type3 @rw_subst_ktyp_type4: sysf_rw.
 
-(** *** <<subst>> with <<KTerm>> *)
+(** *** <<subst>> with <<ktrm>> *)
 (******************************************************************************)
-Section rw_subst_KTerm_type.
+Section rw_subst_ktrm_type.
 
   Context
     (x: atom)
     (u: term LN).
 
-  Lemma rw_subst_KTerm_type1: forall c, subst typ KTerm x u (ty_c c) = ty_c c.
+  Lemma rw_subst_ktrm_type1: forall c, subst typ ktrm x u (ty_c c) = ty_c c.
   Proof. reflexivity. Qed.
 
-  Lemma rw_subst_KTerm_type2: forall (l: LN), subst typ KTerm x u (ty_v l) = ty_v l.
+  Lemma rw_subst_ktrm_type2: forall (l: LN), subst typ ktrm x u (ty_v l) = ty_v l.
   Proof. reflexivity. Qed.
 
-  Lemma rw_subst_KTerm_type3: forall (t1 t2: typ LN), subst typ KTerm x u (ty_ar t1 t2) = ty_ar (subst typ KTerm x u t1) (subst typ KTerm x u t2).
+  Lemma rw_subst_ktrm_type3: forall (t1 t2: typ LN), subst typ ktrm x u (ty_ar t1 t2) = ty_ar (subst typ ktrm x u t1) (subst typ ktrm x u t2).
   Proof. reflexivity. Qed.
 
-  Lemma rw_subst_KTerm_type4: forall (t: typ LN), subst typ KTerm x u (ty_univ t) = ty_univ (subst typ KTerm x u t).
+  Lemma rw_subst_ktrm_type4: forall (t: typ LN), subst typ ktrm x u (ty_univ t) = ty_univ (subst typ ktrm x u t).
   Proof.
     intros.
     unfold subst.
@@ -945,11 +687,11 @@ Section rw_subst_KTerm_type.
     reflexivity.
   Qed.
 
-End rw_subst_KTerm_type.
+End rw_subst_ktrm_type.
 
-#[export] Hint Rewrite @rw_subst_KTerm_type1 @rw_subst_KTerm_type2 @rw_subst_KTerm_type3 @rw_subst_KTerm_type4: sysf_rw.
+#[export] Hint Rewrite @rw_subst_ktrm_type1 @rw_subst_ktrm_type2 @rw_subst_ktrm_type3 @rw_subst_ktrm_type4: sysf_rw.
 
-Corollary rw_subst_KTerm_type: forall (τ: typ LN) (x: atom) (u: term LN), subst typ KTerm x u τ = τ.
+Corollary rw_subst_ktrm_type: forall (τ: typ LN) (x: atom) (u: term LN), subst typ ktrm x u τ = τ.
 Proof.
   intros; induction τ; try easy.
   - cbn. now rewrite IHτ1, IHτ2.
@@ -957,22 +699,22 @@ Proof.
     now rewrite IHτ.
 Qed.
 
-#[export] Hint Rewrite @rw_subst_KTerm_type: sysf_rw.
+#[export] Hint Rewrite @rw_subst_ktrm_type: sysf_rw.
 
-(** *** <<locally_closed>> with <<KType>> *)
+(** *** <<locally_closed>> with <<ktyp>> *)
 (******************************************************************************)
-Section rw_lc_KType_type.
+Section rw_lc_ktyp_type.
 
-  Lemma rw_lc_KType_type1: forall c, locally_closed typ KType (ty_c c).
+  Lemma rw_lc_ktyp_type1: forall c, locally_closed typ ktyp (ty_c c).
   Proof.
     intros. unfold locally_closed, locally_closed_gap; introv hyp.
-    now rewrite rw_tomsetd_type1 in hyp.
+    now rewrite rw_tosetmd_type1 in hyp.
   Qed.
 
-  Lemma rw_lc_KType_type2: forall (l: LN), locally_closed typ KType (ty_v l) <-> exists x, l = Fr x.
+  Lemma rw_lc_ktyp_type2: forall (l: LN), locally_closed typ ktyp (ty_v l) <-> exists x, l = Fr x.
   Proof.
     intros. unfold locally_closed, locally_closed_gap.
-    setoid_rewrite rw_tomsetd_type2. split.
+    setoid_rewrite rw_tosetmd_type2. split.
     - introv hyp. destruct l.
       + eauto.
       + enough (n < 0). lia. now apply (hyp [] (Bd n)).
@@ -980,21 +722,21 @@ Section rw_lc_KType_type.
       inverts H0. cbn; trivial.
   Qed.
 
-  Lemma rw_lc_KType_type3: forall (t1 t2: typ LN), locally_closed typ KType (ty_ar t1 t2) <-> (locally_closed typ KType t1 /\ locally_closed typ KType t2).
+  Lemma rw_lc_ktyp_type3: forall (t1 t2: typ LN), locally_closed typ ktyp (ty_ar t1 t2) <-> (locally_closed typ ktyp t1 /\ locally_closed typ ktyp t2).
   Proof.
     intros. unfold locally_closed, locally_closed_gap.
-    setoid_rewrite rw_tomsetd_type3. firstorder.
+    setoid_rewrite rw_tosetmd_type3. firstorder.
   Qed.
 
   #[local] Open Scope nat_scope.
 
-  Lemma rw_lc_KType_type4: forall (t: typ LN), locally_closed typ KType (ty_univ t) <-> locally_closed_gap typ KType 1 t.
+  Lemma rw_lc_ktyp_type4: forall (t: typ LN), locally_closed typ ktyp (ty_univ t) <-> locally_closed_gap typ ktyp 1 t.
   Proof.
     intros. unfold locally_closed, locally_closed_gap.
-    setoid_rewrite rw_tomsetd_type4. split.
+    setoid_rewrite rw_tosetmd_type4. split.
     - intros hyp w l Hin.
-      specialize (hyp (KType:: w) l). cbn in *.
-      assert (rw: S (countk (@KType: K) w + 0) = (countk KType w + 1)) by lia.
+      specialize (hyp (ktyp:: w) l). cbn in *.
+      assert (rw: S (countk (@ktyp: K) w + 0) = (countk ktyp w + 1)) by lia.
       rewrite <- rw. apply hyp. eauto.
     - intros hyp w l [w' [H1 H2]]. subst.
       specialize (hyp w' l H1). cbn in *. destruct l.
@@ -1002,39 +744,39 @@ Section rw_lc_KType_type.
       + lia.
   Qed.
 
-End rw_lc_KType_type.
+End rw_lc_ktyp_type.
 
-#[export] Hint Rewrite @rw_lc_KType_type1 @rw_lc_KType_type2 @rw_lc_KType_type3 @rw_lc_KType_type4: sysf_rw.
+#[export] Hint Rewrite @rw_lc_ktyp_type1 @rw_lc_ktyp_type2 @rw_lc_ktyp_type3 @rw_lc_ktyp_type4: sysf_rw.
 
-(** *** <<locally_closed>> with <<KTerm>> *)
+(** *** <<locally_closed>> with <<ktrm>> *)
 (******************************************************************************)
-Section rw_lc_KTerm_type.
+Section rw_lc_ktrm_type.
 
-  Lemma rw_lc_KTerm_type: forall τ, locally_closed typ KTerm τ <-> True.
+  Lemma rw_lc_ktrm_type: forall τ, locally_closed typ ktrm τ <-> True.
   Proof.
     intros. unfold locally_closed, locally_closed_gap.
-    setoid_rewrite rw_tomsetd_type_KTerm. intuition.
+    setoid_rewrite rw_tosetmd_type_ktrm. intuition.
   Qed.
 
-  Lemma lc_KTerm_type: forall τ, locally_closed typ KTerm τ.
+  Lemma lc_ktrm_type: forall τ, locally_closed typ ktrm τ.
   Proof.
-    intros. now rewrite rw_lc_KTerm_type.
+    intros. now rewrite rw_lc_ktrm_type.
   Qed.
 
-End rw_lc_KTerm_type.
+End rw_lc_ktrm_type.
 
-#[export] Hint Rewrite @rw_lc_KTerm_type: sysf_rw.
+#[export] Hint Rewrite @rw_lc_ktrm_type: sysf_rw.
 
-(** *** <<scoped>> with <<KTerm>> *)
+(** *** <<scoped>> with <<ktrm>> *)
 (******************************************************************************)
-Section rw_scoped_KTerm_type.
+Section rw_scoped_ktrm_type.
 
-  Lemma rw_scoped_KTerm_type: forall τ (vars: AtomSet.t), scoped typ KTerm τ vars.
+  Lemma rw_scoped_ktrm_type: forall τ (vars: Atosetm.t), scoped typ ktrm τ vars.
   Proof.
     intros. unfold scoped. autorewrite with sysf_rw. fsetdec.
   Qed.
 
-End rw_scoped_KTerm_type.
+End rw_scoped_ktrm_type.
 
 (** ** <<ok_type>> *)
 (******************************************************************************)
@@ -1050,8 +792,8 @@ Qed.
 
 Lemma ok_type_univ: forall Δ τ,
     ok_type Δ (ty_univ τ) <->
-    scoped typ KType τ (AssocList.domset Δ) /\
-    locally_closed_gap typ KType 1 τ.
+    scoped typ ktyp τ (AssocList.domset Δ) /\
+    locally_closed_gap typ ktyp 1 τ.
 Proof.
   intros. unfold ok_type.
   unfold scoped.
@@ -1075,16 +817,16 @@ Section rw_mmapdt_term.
     `{Applicative F}
     (f: K -> list K * A -> F B).
 
-  Lemma rw_mmapdt_term1: forall (a: A), mmapdt term F f (tm_var a) = pure tm_var <⋆> f KTerm (nil, a).
+  Lemma rw_mmapdt_term1: forall (a: A), mmapdt term F f (tm_var a) = pure tm_var <⋆> f ktrm (nil, a).
   Proof. intros. unfold mmapdt. autorewrite with sysf_rw. now rewrite <- map_to_ap. Qed.
 
-  Lemma rw_mmapdt_term2: forall (τ: typ A) (t: term A), mmapdt term F f (tm_abs τ t) = pure tm_abs <⋆> (mmapdt typ F f τ) <⋆> (mmapdt term F (fun k => f k ∘ incr [KTerm]) t).
+  Lemma rw_mmapdt_term2: forall (τ: typ A) (t: term A), mmapdt term F f (tm_abs τ t) = pure tm_abs <⋆> (mmapdt typ F f τ) <⋆> (mmapdt term F (fun k => f k ∘ incr [ktrm]) t).
   Proof. reflexivity. Qed.
 
   Lemma rw_mmapdt_term3: forall (t1 t2: term A), mmapdt term F f (tm_app t1 t2) = pure tm_app <⋆> (mmapdt term F f t1) <⋆> (mmapdt term F f t2).
   Proof. reflexivity. Qed.
 
-  Lemma rw_mmapdt_term4: forall (t: term A), mmapdt term F f (tm_tab t) = pure tm_tab <⋆> (mmapdt term F (fun k => f k ∘ incr [KType]) t).
+  Lemma rw_mmapdt_term4: forall (t: term A), mmapdt term F f (tm_tab t) = pure tm_tab <⋆> (mmapdt term F (fun k => f k ∘ incr [ktyp]) t).
   Proof. reflexivity. Qed.
 
   Lemma rw_mmapdt_term5: forall (t: term A) (τ: typ A), mmapdt term F f (tm_tap t τ) = pure tm_tap <⋆> (mmapdt term F f t) <⋆> (mmapdt typ F f τ).
@@ -1102,16 +844,16 @@ Section rw_mbindd_term.
     (A B: Type)
     (f: forall k, list K * A -> SystemF k B).
 
-  Lemma rw_mbindd_term1: forall (a: A), mbindd term f (tm_var a) = f KTerm (nil, a).
+  Lemma rw_mbindd_term1: forall (a: A), mbindd term f (tm_var a) = f ktrm (nil, a).
   Proof. reflexivity. Qed.
 
-  Lemma rw_mbindd_term2: forall (τ: typ A) (t: term A), mbindd term f (tm_abs τ t) = tm_abs (mbindd typ f τ) (mbindd term (fun k => f k ∘ incr [KTerm]) t).
+  Lemma rw_mbindd_term2: forall (τ: typ A) (t: term A), mbindd term f (tm_abs τ t) = tm_abs (mbindd typ f τ) (mbindd term (fun k => f k ∘ incr [ktrm]) t).
   Proof. reflexivity. Qed.
 
   Lemma rw_mbindd_term3: forall (t1 t2: term A), mbindd term f (tm_app t1 t2) = tm_app (mbindd term f t1) (mbindd term f t2).
   Proof. reflexivity. Qed.
 
-  Lemma rw_mbindd_term4: forall (t: term A), mbindd term f (tm_tab t) = tm_tab (mbindd term (fun k => f k ∘ incr [KType]) t).
+  Lemma rw_mbindd_term4: forall (t: term A), mbindd term f (tm_tab t) = tm_tab (mbindd term (fun k => f k ∘ incr [ktyp]) t).
   Proof. reflexivity. Qed.
 
   Lemma rw_mbindd_term5: forall (t: term A) (τ: typ A), mbindd term f (tm_tap t τ) = tm_tap (mbindd term f t) (mbindd typ f τ).
@@ -1129,7 +871,7 @@ Section rw_mbind_term.
     (A B: Type)
     (f: forall k, A -> SystemF k B).
 
-  Lemma rw_mbind_term1: forall (a: A), mbind term f (tm_var a) = f KTerm a.
+  Lemma rw_mbind_term1: forall (a: A), mbind term f (tm_var a) = f ktrm a.
   Proof. reflexivity. Qed.
 
   Lemma rw_mbind_term2: forall (τ: typ A) (t: term A), mbind term f (tm_abs τ t) = tm_abs (mbind typ f τ) (mbind term f t).
@@ -1148,235 +890,235 @@ End rw_mbind_term.
 
 #[export] Hint Rewrite @rw_mbind_term1 @rw_mbind_term2 @rw_mbind_term3 @rw_mbind_term4 @rw_mbind_term5: sysf_rw.
 
-(** *** <<kbindd>> with <<KType>> *)
+(** *** <<kbindd>> with <<ktyp>> *)
 (******************************************************************************)
-Section rw_kbindd_KType_term.
+Section rw_kbindd_ktyp_term.
 
   Context
     (A: Type)
     (f: list K * A -> typ A).
 
-  Lemma rw_kbindd_KType_term1: forall (a: A), kbindd term KType f (tm_var a) = tm_var a.
+  Lemma rw_kbindd_ktyp_term1: forall (a: A), kbindd term ktyp f (tm_var a) = tm_var a.
   Proof. reflexivity. Qed.
 
-  Lemma rw_kbindd_KType_term2: forall (τ: typ A) (t: term A), kbindd term KType f (tm_abs τ t) = tm_abs (kbindd typ KType f τ) (kbindd term KType (f ∘ incr [KTerm]) t).
+  Lemma rw_kbindd_ktyp_term2: forall (τ: typ A) (t: term A), kbindd term ktyp f (tm_abs τ t) = tm_abs (kbindd typ ktyp f τ) (kbindd term ktyp (f ∘ incr [ktrm]) t).
   Proof. intros. unfold kbindd. autorewrite with sysf_rw. do 2 fequal. now ext k [w a]. Qed.
 
-  Lemma rw_kbindd_KType_term3: forall (t1 t2: term A), kbindd term KType f (tm_app t1 t2) = tm_app (kbindd term KType f t1) (kbindd term KType f t2).
+  Lemma rw_kbindd_ktyp_term3: forall (t1 t2: term A), kbindd term ktyp f (tm_app t1 t2) = tm_app (kbindd term ktyp f t1) (kbindd term ktyp f t2).
   Proof. reflexivity. Qed.
 
-  Lemma rw_kbindd_KType_term4: forall (t: term A), kbindd term KType f (tm_tab t) = tm_tab (kbindd term KType (f ∘ incr [KType]) t).
+  Lemma rw_kbindd_ktyp_term4: forall (t: term A), kbindd term ktyp f (tm_tab t) = tm_tab (kbindd term ktyp (f ∘ incr [ktyp]) t).
   Proof. intros. unfold kbindd. autorewrite with sysf_rw. do 2 fequal. now ext k [w a]. Qed.
 
-  Lemma rw_kbindd_KType_term5: forall (t: term A) (τ: typ A), kbindd term KType f (tm_tap t τ) = tm_tap (kbindd term KType f t) (kbindd typ KType f τ).
+  Lemma rw_kbindd_ktyp_term5: forall (t: term A) (τ: typ A), kbindd term ktyp f (tm_tap t τ) = tm_tap (kbindd term ktyp f t) (kbindd typ ktyp f τ).
   Proof. reflexivity. Qed.
 
-End rw_kbindd_KType_term.
+End rw_kbindd_ktyp_term.
 
-#[export] Hint Rewrite @rw_kbindd_KType_term1 @rw_kbindd_KType_term2 @rw_kbindd_KType_term3 @rw_kbindd_KType_term4 @rw_kbindd_KType_term5: sysf_rw.
+#[export] Hint Rewrite @rw_kbindd_ktyp_term1 @rw_kbindd_ktyp_term2 @rw_kbindd_ktyp_term3 @rw_kbindd_ktyp_term4 @rw_kbindd_ktyp_term5: sysf_rw.
 
-(** *** <<kbindd>> with <<KTerm>> *)
+(** *** <<kbindd>> with <<ktrm>> *)
 (******************************************************************************)
-Section rw_kbindd_KTerm_term.
+Section rw_kbindd_ktrm_term.
 
   Context
     (A: Type)
     (f: list K * A -> term A).
 
-  Lemma rw_kbindd_KTerm_term1: forall (a: A), kbindd term KTerm f (tm_var a) = f (nil, a).
+  Lemma rw_kbindd_ktrm_term1: forall (a: A), kbindd term ktrm f (tm_var a) = f (nil, a).
   Proof. reflexivity. Qed.
 
-  Lemma rw_kbindd_KTerm_term2: forall (τ: typ A) (t: term A), kbindd term KTerm f (tm_abs τ t) = tm_abs (kbindd typ KTerm f τ) (kbindd term KTerm (f ∘ incr [KTerm]) t).
+  Lemma rw_kbindd_ktrm_term2: forall (τ: typ A) (t: term A), kbindd term ktrm f (tm_abs τ t) = tm_abs (kbindd typ ktrm f τ) (kbindd term ktrm (f ∘ incr [ktrm]) t).
   Proof. intros. unfold kbindd. autorewrite with sysf_rw. do 2 fequal. now ext k [w a]. Qed.
 
-  Lemma rw_kbindd_KTerm_term3: forall (t1 t2: term A), kbindd term KTerm f (tm_app t1 t2) = tm_app (kbindd term KTerm f t1) (kbindd term KTerm f t2).
+  Lemma rw_kbindd_ktrm_term3: forall (t1 t2: term A), kbindd term ktrm f (tm_app t1 t2) = tm_app (kbindd term ktrm f t1) (kbindd term ktrm f t2).
   Proof. reflexivity. Qed.
 
-  Lemma rw_kbindd_KTerm_term4: forall (t: term A), kbindd term KTerm f (tm_tab t) = tm_tab (kbindd term KTerm (f ∘ incr [KType]) t).
+  Lemma rw_kbindd_ktrm_term4: forall (t: term A), kbindd term ktrm f (tm_tab t) = tm_tab (kbindd term ktrm (f ∘ incr [ktyp]) t).
   Proof. intros. unfold kbindd. autorewrite with sysf_rw. do 2 fequal. now ext k [w a]. Qed.
 
-  Lemma rw_kbindd_KTerm_term5: forall (t: term A) (τ: typ A), kbindd term KTerm f (tm_tap t τ) = tm_tap (kbindd term KTerm f t) (kbindd typ KTerm f τ).
+  Lemma rw_kbindd_ktrm_term5: forall (t: term A) (τ: typ A), kbindd term ktrm f (tm_tap t τ) = tm_tap (kbindd term ktrm f t) (kbindd typ ktrm f τ).
   Proof. reflexivity. Qed.
 
-End rw_kbindd_KTerm_term.
+End rw_kbindd_ktrm_term.
 
-#[export] Hint Rewrite @rw_kbindd_KTerm_term1 @rw_kbindd_KTerm_term2 @rw_kbindd_KTerm_term3 @rw_kbindd_KTerm_term4 @rw_kbindd_KTerm_term5: sysf_rw.
+#[export] Hint Rewrite @rw_kbindd_ktrm_term1 @rw_kbindd_ktrm_term2 @rw_kbindd_ktrm_term3 @rw_kbindd_ktrm_term4 @rw_kbindd_ktrm_term5: sysf_rw.
 
-(** *** <<kbind>> with <<KType>> *)
+(** *** <<kbind>> with <<ktyp>> *)
 (******************************************************************************)
-Section rw_kbind_KType_term.
+Section rw_kbind_ktyp_term.
 
   Context
     (A: Type)
     (f: A -> typ A).
 
-  Lemma rw_kbind_KType_term1: forall (a: A), kbind term KType f (tm_var a) = tm_var a.
+  Lemma rw_kbind_ktyp_term1: forall (a: A), kbind term ktyp f (tm_var a) = tm_var a.
   Proof. reflexivity. Qed.
 
-  Lemma rw_kbind_KType_term2: forall (τ: typ A) (t: term A), kbind term KType f (tm_abs τ t) = tm_abs (kbind typ KType f τ) (kbind term KType f t).
+  Lemma rw_kbind_ktyp_term2: forall (τ: typ A) (t: term A), kbind term ktyp f (tm_abs τ t) = tm_abs (kbind typ ktyp f τ) (kbind term ktyp f t).
   Proof. intros. unfold kbind. now autorewrite with sysf_rw. Qed.
 
-  Lemma rw_kbind_KType_term3: forall (t1 t2: term A), kbind term KType f (tm_app t1 t2) = tm_app (kbind term KType f t1) (kbind term KType f t2).
+  Lemma rw_kbind_ktyp_term3: forall (t1 t2: term A), kbind term ktyp f (tm_app t1 t2) = tm_app (kbind term ktyp f t1) (kbind term ktyp f t2).
   Proof. reflexivity. Qed.
 
-  Lemma rw_kbind_KType_term4: forall (t: term A), kbind term KType f (tm_tab t) = tm_tab (kbind term KType f t).
+  Lemma rw_kbind_ktyp_term4: forall (t: term A), kbind term ktyp f (tm_tab t) = tm_tab (kbind term ktyp f t).
   Proof. intros. unfold kbind. now autorewrite with sysf_rw. Qed.
 
-  Lemma rw_kbind_KType_term5: forall (t: term A) (τ: typ A), kbind term KType f (tm_tap t τ) = tm_tap (kbind term KType f t) (kbind typ KType f τ).
+  Lemma rw_kbind_ktyp_term5: forall (t: term A) (τ: typ A), kbind term ktyp f (tm_tap t τ) = tm_tap (kbind term ktyp f t) (kbind typ ktyp f τ).
   Proof. reflexivity. Qed.
 
-End rw_kbind_KType_term.
+End rw_kbind_ktyp_term.
 
-#[export] Hint Rewrite @rw_kbind_KType_term1 @rw_kbind_KType_term2 @rw_kbind_KType_term3 @rw_kbind_KType_term4 @rw_kbind_KType_term5: sysf_rw.
+#[export] Hint Rewrite @rw_kbind_ktyp_term1 @rw_kbind_ktyp_term2 @rw_kbind_ktyp_term3 @rw_kbind_ktyp_term4 @rw_kbind_ktyp_term5: sysf_rw.
 
-(** *** <<kbind>> with <<KTerm>> *)
+(** *** <<kbind>> with <<ktrm>> *)
 (******************************************************************************)
-Section rw_kbind_KTerm_term.
+Section rw_kbind_ktrm_term.
 
   Context
     (A: Type)
     (f: A -> term A).
 
-  Lemma rw_kbind_KTerm_term1: forall (a: A), kbind term KTerm f (tm_var a) = f a.
+  Lemma rw_kbind_ktrm_term1: forall (a: A), kbind term ktrm f (tm_var a) = f a.
   Proof. reflexivity. Qed.
 
-  Lemma rw_kbind_KTerm_term2: forall (τ: typ A) (t: term A), kbind term KTerm f (tm_abs τ t) = tm_abs (kbind typ KTerm f τ) (kbind term KTerm f t).
+  Lemma rw_kbind_ktrm_term2: forall (τ: typ A) (t: term A), kbind term ktrm f (tm_abs τ t) = tm_abs (kbind typ ktrm f τ) (kbind term ktrm f t).
   Proof. intros. unfold kbind. now autorewrite with sysf_rw. Qed.
 
-  Lemma rw_kbind_KTerm_term3: forall (t1 t2: term A), kbind term KTerm f (tm_app t1 t2) = tm_app (kbind term KTerm f t1) (kbind term KTerm f t2).
+  Lemma rw_kbind_ktrm_term3: forall (t1 t2: term A), kbind term ktrm f (tm_app t1 t2) = tm_app (kbind term ktrm f t1) (kbind term ktrm f t2).
   Proof. reflexivity. Qed.
 
-  Lemma rw_kbind_KTerm_term4: forall (t: term A), kbind term KTerm f (tm_tab t) = tm_tab (kbind term KTerm f t).
+  Lemma rw_kbind_ktrm_term4: forall (t: term A), kbind term ktrm f (tm_tab t) = tm_tab (kbind term ktrm f t).
   Proof. intros. unfold kbind. now autorewrite with sysf_rw. Qed.
 
-  Lemma rw_kbind_KTerm_term5: forall (t: term A) (τ: typ A), kbind term KTerm f (tm_tap t τ) = tm_tap (kbind term KTerm f t) (kbind typ KTerm f τ).
+  Lemma rw_kbind_ktrm_term5: forall (t: term A) (τ: typ A), kbind term ktrm f (tm_tap t τ) = tm_tap (kbind term ktrm f t) (kbind typ ktrm f τ).
   Proof. reflexivity. Qed.
 
-End rw_kbind_KTerm_term.
+End rw_kbind_ktrm_term.
 
-#[export] Hint Rewrite @rw_kbind_KTerm_term1 @rw_kbind_KTerm_term2 @rw_kbind_KTerm_term3 @rw_kbind_KTerm_term4 @rw_kbind_KTerm_term5: sysf_rw.
+#[export] Hint Rewrite @rw_kbind_ktrm_term1 @rw_kbind_ktrm_term2 @rw_kbind_ktrm_term3 @rw_kbind_ktrm_term4 @rw_kbind_ktrm_term5: sysf_rw.
 
 (** ** List and occurrence operations *)
 (******************************************************************************)
 
-(** *** <<tomlistd>> *)
+(** *** <<tolistmd>> *)
 (******************************************************************************)
-Section rw_tomlistd_type.
+Section rw_tolistmd_type.
 
   Context
     (A: Type).
 
   Implicit Types (τ: typ A) (t: term A) (a: A).
 
-  Lemma rw_tomlistd_term1: forall (a: A), tomlistd term (tm_var a) = [ (nil, (KTerm, a)) ].
+  Lemma rw_tolistmd_term1: forall (a: A), tolistmd term (tm_var a) = [ (nil, (ktrm, a)) ].
   Proof. reflexivity. Qed.
 
-  Lemma rw_tomlistd_term2: forall τ t, tomlistd term (tm_abs τ t) = tomlistd typ τ ++ map (F:= list) (incr [KTerm]) (tomlistd term t).
+  Lemma rw_tolistmd_term2: forall τ t, tolistmd term (tm_abs τ t) = tolistmd typ τ ++ map (F:= list) (incr [ktrm]) (tolistmd term t).
   Proof.
-    intros. unfold tomlistd, tomlistd_gen. rewrite rw_mmapdt_term2. fequal.
+    intros. unfold tolistmd, tolistmd_gen. rewrite rw_mmapdt_term2. fequal.
     compose near t on right. unfold mmapdt.
     rewrite (dtp_mbinddt_morphism
                (list (@K I2)) term SystemF (const (list (list K2 * (K * A))))
-               (const (list _)) (ϕ:= (fun _ => map (F:= list) (incr [KTerm])))
+               (const (list _)) (ϕ:= (fun _ => map (F:= list) (incr [ktrm])))
                (fun (k: @K I2) => map (F:= const (list (list K2 * (K * A))))
                                   (mret SystemF k) ∘ (fun '(w, a) => [(w, (k, a))]))).
     fequal. now ext k [w a].
   Qed.
 
-  Lemma rw_tomlistd_term3: forall t1 t2, tomlistd term (tm_app t1 t2) = tomlistd term t1 ++ tomlistd term t2.
+  Lemma rw_tolistmd_term3: forall t1 t2, tolistmd term (tm_app t1 t2) = tolistmd term t1 ++ tolistmd term t2.
   Proof. reflexivity. Qed.
 
-  Lemma rw_tomlistd_term4: forall t, tomlistd term (tm_tab t) = map (F:= list) (incr [KType]) (tomlistd term t).
+  Lemma rw_tolistmd_term4: forall t, tolistmd term (tm_tab t) = map (F:= list) (incr [ktyp]) (tolistmd term t).
   Proof.
-    intros. unfold tomlistd, tomlistd_gen.
+    intros. unfold tolistmd, tolistmd_gen.
     rewrite rw_mmapdt_term4. cbn.
     compose near t on right. unfold mmapdt.
     rewrite (dtp_mbinddt_morphism
-               (list (@K I2)) term SystemF (const (list _)) (const (list _)) (ϕ:= (fun _ => map (F:= list) (incr [KType])))
+               (list (@K I2)) term SystemF (const (list _)) (const (list _)) (ϕ:= (fun _ => map (F:= list) (incr [ktyp])))
                (fun (k: @K I2) => map (F:= const (list (list K2 * (K2 * A)))) (mret SystemF k) ∘ (fun '(w, a) => [(w, (k, a))]))).
     fequal. now ext k [w a].
   Qed.
 
-  Lemma rw_tomlistd_term5: forall t τ, tomlistd term (tm_tap t τ) = tomlistd term t ++ tomlistd typ τ.
+  Lemma rw_tolistmd_term5: forall t τ, tolistmd term (tm_tap t τ) = tolistmd term t ++ tolistmd typ τ.
   Proof. reflexivity. Qed.
 
-End rw_tomlistd_type.
+End rw_tolistmd_type.
 
-#[export] Hint Rewrite @rw_tomlistd_term1 @rw_tomlistd_term2 @rw_tomlistd_term3 @rw_tomlistd_term4 @rw_tomlistd_term5: sysf_rw.
+#[export] Hint Rewrite @rw_tolistmd_term1 @rw_tolistmd_term2 @rw_tolistmd_term3 @rw_tolistmd_term4 @rw_tolistmd_term5: sysf_rw.
 
-(** *** <<toklistd>> with <<KType>> *)
+(** *** <<toklistd>> with <<ktyp>> *)
 (******************************************************************************)
-Section rw_toklistd_KType_type.
+Section rw_toklistd_ktyp_type.
 
   Context
     (A: Type).
 
   Implicit Types (τ: typ A) (t: term A) (a: A).
 
-  Lemma rw_toklistd_KType_term1: forall (a: A), toklistd term KType (tm_var a) = nil.
+  Lemma rw_toklistd_ktyp_term1: forall (a: A), toklistd term ktyp (tm_var a) = nil.
   Proof. reflexivity. Qed.
 
-  Lemma rw_toklistd_KType_term2: forall τ t, toklistd term KType (tm_abs τ t) = toklistd typ KType τ ++ map (F:= list) (incr [KTerm]) (toklistd term KType t).
-  Proof. intros. unfold toklistd, compose. rewrite rw_tomlistd_term2. rewrite filterk_app. now rewrite filterk_incr. Qed.
+  Lemma rw_toklistd_ktyp_term2: forall τ t, toklistd term ktyp (tm_abs τ t) = toklistd typ ktyp τ ++ map (F:= list) (incr [ktrm]) (toklistd term ktyp t).
+  Proof. intros. unfold toklistd, compose. rewrite rw_tolistmd_term2. rewrite filterk_app. now rewrite filterk_incr. Qed.
 
-  Lemma rw_toklistd_KType_term3: forall t1 t2, toklistd term KType (tm_app t1 t2) = toklistd term KType t1 ++ toklistd term KType t2.
+  Lemma rw_toklistd_ktyp_term3: forall t1 t2, toklistd term ktyp (tm_app t1 t2) = toklistd term ktyp t1 ++ toklistd term ktyp t2.
   Proof. intros. unfold toklistd, compose. autorewrite with sysf_rw. now rewrite filterk_app. Qed.
 
-  Lemma rw_toklistd_KType_term4: forall t, toklistd term KType (tm_tab t) = map (F:= list) (incr [KType]) (toklistd term KType t).
+  Lemma rw_toklistd_ktyp_term4: forall t, toklistd term ktyp (tm_tab t) = map (F:= list) (incr [ktyp]) (toklistd term ktyp t).
   Proof. intros. unfold toklistd, compose. autorewrite with sysf_rw. now rewrite filterk_incr. Qed.
 
-  Lemma rw_toklistd_KType_term5: forall t τ, toklistd term KType (tm_tap t τ) = toklistd term KType t ++ toklistd typ KType τ.
+  Lemma rw_toklistd_ktyp_term5: forall t τ, toklistd term ktyp (tm_tap t τ) = toklistd term ktyp t ++ toklistd typ ktyp τ.
   Proof. intros. unfold toklistd, compose. autorewrite with sysf_rw. now rewrite filterk_app. Qed.
 
-End rw_toklistd_KType_type.
+End rw_toklistd_ktyp_type.
 
-#[export] Hint Rewrite @rw_toklistd_KType_term1 @rw_toklistd_KType_term2 @rw_toklistd_KType_term3 @rw_toklistd_KType_term4 @rw_toklistd_KType_term5: sysf_rw.
+#[export] Hint Rewrite @rw_toklistd_ktyp_term1 @rw_toklistd_ktyp_term2 @rw_toklistd_ktyp_term3 @rw_toklistd_ktyp_term4 @rw_toklistd_ktyp_term5: sysf_rw.
 
-(** *** <<toklistd>> with <<KTerm>> *)
+(** *** <<toklistd>> with <<ktrm>> *)
 (******************************************************************************)
-Section rw_toklistd_KTerm_term.
+Section rw_toklistd_ktrm_term.
 
   Context
     (A: Type).
 
   Implicit Types (τ: typ A) (t: term A) (a: A).
 
-  Lemma rw_toklistd_KTerm_term1: forall (a: A), toklistd term KTerm (tm_var a) = [ (nil, a) ].
+  Lemma rw_toklistd_ktrm_term1: forall (a: A), toklistd term ktrm (tm_var a) = [ (nil, a) ].
   Proof. reflexivity. Qed.
 
-  Lemma rw_toklistd_KTerm_term2: forall τ t, toklistd term KTerm (tm_abs τ t) = toklistd typ KTerm τ ++ map (F:= list) (incr [KTerm]) (toklistd term KTerm t).
-  Proof. intros. unfold toklistd, compose. rewrite rw_tomlistd_term2. rewrite filterk_app. now rewrite filterk_incr. Qed.
+  Lemma rw_toklistd_ktrm_term2: forall τ t, toklistd term ktrm (tm_abs τ t) = toklistd typ ktrm τ ++ map (F:= list) (incr [ktrm]) (toklistd term ktrm t).
+  Proof. intros. unfold toklistd, compose. rewrite rw_tolistmd_term2. rewrite filterk_app. now rewrite filterk_incr. Qed.
 
-  Lemma rw_toklistd_KTerm_term3: forall t1 t2, toklistd term KTerm (tm_app t1 t2) = toklistd term KTerm t1 ++ toklistd term KTerm t2.
+  Lemma rw_toklistd_ktrm_term3: forall t1 t2, toklistd term ktrm (tm_app t1 t2) = toklistd term ktrm t1 ++ toklistd term ktrm t2.
   Proof. intros. unfold toklistd, compose. autorewrite with sysf_rw. now rewrite filterk_app. Qed.
 
-  Lemma rw_toklistd_KTerm_term4: forall t, toklistd term KTerm (tm_tab t) = map (F:= list) (incr [KType]) (toklistd term KTerm t).
+  Lemma rw_toklistd_ktrm_term4: forall t, toklistd term ktrm (tm_tab t) = map (F:= list) (incr [ktyp]) (toklistd term ktrm t).
   Proof. intros. unfold toklistd, compose. autorewrite with sysf_rw. now rewrite filterk_incr. Qed.
 
-  Lemma rw_toklistd_KTerm_term5: forall t τ, toklistd term KTerm (tm_tap t τ) = toklistd term KTerm t ++ toklistd typ KTerm τ.
+  Lemma rw_toklistd_ktrm_term5: forall t τ, toklistd term ktrm (tm_tap t τ) = toklistd term ktrm t ++ toklistd typ ktrm τ.
   Proof. intros. unfold toklistd, compose. autorewrite with sysf_rw. now rewrite filterk_app. Qed.
 
-End rw_toklistd_KTerm_term.
+End rw_toklistd_ktrm_term.
 
-#[export] Hint Rewrite @rw_toklistd_KTerm_term1 @rw_toklistd_KTerm_term2 @rw_toklistd_KTerm_term3 @rw_toklistd_KTerm_term4 @rw_toklistd_KTerm_term5: sysf_rw.
+#[export] Hint Rewrite @rw_toklistd_ktrm_term1 @rw_toklistd_ktrm_term2 @rw_toklistd_ktrm_term3 @rw_toklistd_ktrm_term4 @rw_toklistd_ktrm_term5: sysf_rw.
 
-(** *** <<tomlist>> *)
+(** *** <<tolistm>> *)
 (******************************************************************************)
-Section rw_tomlist_term.
+Section rw_tolistm_term.
 
   Context
     (A: Type).
 
   Implicit Types (τ: typ A) (t: term A) (a: A).
 
-  Lemma rw_tomlist_term1: forall (a: A), tomlist term (tm_var a) = [ (KTerm, a) ].
+  Lemma rw_tolistm_term1: forall (a: A), tolistm term (tm_var a) = [ (ktrm, a) ].
   Proof. reflexivity. Qed.
 
-  Lemma rw_tomlist_term2: forall τ t, tomlist term (tm_abs τ t) = tomlist typ τ ++ tomlist term t.
+  Lemma rw_tolistm_term2: forall τ t, tolistm term (tm_abs τ t) = tolistm typ τ ++ tolistm term t.
   Proof.
     intros.
-    unfold tomlist, tomlistd.
-    unfold tomlistd_gen.
+    unfold tolistm, tolistmd.
+    unfold tolistmd_gen.
     unfold compose.
     rewrite mmapdt_to_mbinddt.
     rewrite mmapdt_to_mbinddt.
@@ -1392,105 +1134,105 @@ Section rw_tomlist_term.
 
     (*
     autorewrite with sysf_rw tea_list.
-    compose near (tomlistd term t) on left. rewrite (fun_map_map (F:= list)).
+    compose near (tolistmd term t) on left. rewrite (fun_map_map (F:= list)).
     repeat fequal. now ext [w a].
   Qed.
      *)
   Admitted.
 
-  Lemma rw_tomlist_term3: forall t1 t2, tomlist term (tm_app t1 t2) = tomlist term t1 ++ tomlist term t2.
-  Proof. intros. unfold tomlist, compose. now autorewrite with sysf_rw tea_list. Qed.
+  Lemma rw_tolistm_term3: forall t1 t2, tolistm term (tm_app t1 t2) = tolistm term t1 ++ tolistm term t2.
+  Proof. intros. unfold tolistm, compose. now autorewrite with sysf_rw tea_list. Qed.
 
-  Lemma rw_tomlist_term4: forall t, tomlist term (tm_tab t) = tomlist term t.
+  Lemma rw_tolistm_term4: forall t, tolistm term (tm_tab t) = tolistm term t.
   Proof.
-    intros. unfold tomlist, compose. autorewrite with sysf_rw.
-    compose near (tomlistd term t) on left. rewrite (fun_map_map (F:= list)).
+    intros. unfold tolistm, compose. autorewrite with sysf_rw.
+    compose near (tolistmd term t) on left. rewrite (fun_map_map (F:= list)).
     repeat fequal. now ext [w a].
   Qed.
 
-  Lemma rw_tomlist_term5: forall t τ, tomlist term (tm_tap t τ) = tomlist term t ++ tomlist typ τ.
-  Proof. intros. unfold tomlist, compose. now autorewrite with sysf_rw tea_list. Qed.
+  Lemma rw_tolistm_term5: forall t τ, tolistm term (tm_tap t τ) = tolistm term t ++ tolistm typ τ.
+  Proof. intros. unfold tolistm, compose. now autorewrite with sysf_rw tea_list. Qed.
 
-End rw_tomlist_term.
+End rw_tolistm_term.
 
-#[export] Hint Rewrite @rw_tomlist_term1 @rw_tomlist_term2 @rw_tomlist_term3 @rw_tomlist_term4 @rw_tomlist_term5: sysf_rw.
+#[export] Hint Rewrite @rw_tolistm_term1 @rw_tolistm_term2 @rw_tolistm_term3 @rw_tolistm_term4 @rw_tolistm_term5: sysf_rw.
 
-(** *** <<toklist>> with <<KType>> *)
+(** *** <<toklist>> with <<ktyp>> *)
 (******************************************************************************)
-Section rw_toklist_KType_term.
+Section rw_toklist_ktyp_term.
 
   Context
     (A: Type).
 
   Implicit Types (τ: typ A) (t: term A) (a: A).
 
-  Lemma rw_toklist_KType_term1: forall (a: A), toklist term KType (tm_var a) = [ ].
+  Lemma rw_toklist_ktyp_term1: forall (a: A), toklist term ktyp (tm_var a) = [ ].
   Proof. reflexivity. Qed.
 
-  Lemma rw_toklist_KType_term2: forall τ t, toklist term KType (tm_abs τ t) = toklist typ KType τ ++ toklist term KType t.
+  Lemma rw_toklist_ktyp_term2: forall τ t, toklist term ktyp (tm_abs τ t) = toklist typ ktyp τ ++ toklist term ktyp t.
   Proof.
     intros. unfold toklist, compose.
     autorewrite with sysf_rw tea_list.
-    compose near (toklistd term KType t) on left. rewrite (fun_map_map (F:= list)).
+    compose near (toklistd term ktyp t) on left. rewrite (fun_map_map (F:= list)).
     repeat fequal. now ext [w a].
   Qed.
 
-  Lemma rw_toklist_KType_term3: forall t1 t2, toklist term KType (tm_app t1 t2) = toklist term KType t1 ++ toklist term KType t2.
+  Lemma rw_toklist_ktyp_term3: forall t1 t2, toklist term ktyp (tm_app t1 t2) = toklist term ktyp t1 ++ toklist term ktyp t2.
   Proof. intros. unfold toklist, compose. now autorewrite with sysf_rw tea_list. Qed.
 
-  Lemma rw_toklist_KType_term4: forall t, toklist term KType (tm_tab t) = toklist term KType t.
+  Lemma rw_toklist_ktyp_term4: forall t, toklist term ktyp (tm_tab t) = toklist term ktyp t.
   Proof.
     intros. unfold toklist, compose. autorewrite with sysf_rw.
-    compose near (toklistd term KType t) on left. rewrite (fun_map_map (F:= list)).
+    compose near (toklistd term ktyp t) on left. rewrite (fun_map_map (F:= list)).
     repeat fequal. now ext [w a].
   Qed.
 
-  Lemma rw_toklist_KType_term5: forall t τ, toklist term KType (tm_tap t τ) = toklist term KType t ++ toklist typ KType τ.
+  Lemma rw_toklist_ktyp_term5: forall t τ, toklist term ktyp (tm_tap t τ) = toklist term ktyp t ++ toklist typ ktyp τ.
   Proof. intros. unfold toklist, compose. now autorewrite with sysf_rw tea_list. Qed.
 
-End rw_toklist_KType_term.
+End rw_toklist_ktyp_term.
 
-#[export] Hint Rewrite @rw_toklist_KType_term1 @rw_toklist_KType_term2 @rw_toklist_KType_term3 @rw_toklist_KType_term4 @rw_toklist_KType_term5: sysf_rw.
+#[export] Hint Rewrite @rw_toklist_ktyp_term1 @rw_toklist_ktyp_term2 @rw_toklist_ktyp_term3 @rw_toklist_ktyp_term4 @rw_toklist_ktyp_term5: sysf_rw.
 
-(** *** <<toklist>> with <<KTerm>> *)
+(** *** <<toklist>> with <<ktrm>> *)
 (******************************************************************************)
-Section rw_toklist_KTerm_term.
+Section rw_toklist_ktrm_term.
 
   Context
     (A: Type).
 
   Implicit Types (τ: typ A) (t: term A) (a: A).
 
-  Lemma rw_toklist_KTerm_term1: forall (a: A), toklist term KTerm (tm_var a) = [ a ].
+  Lemma rw_toklist_ktrm_term1: forall (a: A), toklist term ktrm (tm_var a) = [ a ].
   Proof. reflexivity. Qed.
 
-  Lemma rw_toklist_KTerm_term2: forall τ t, toklist term KTerm (tm_abs τ t) = toklist typ KTerm τ ++ toklist term KTerm t.
+  Lemma rw_toklist_ktrm_term2: forall τ t, toklist term ktrm (tm_abs τ t) = toklist typ ktrm τ ++ toklist term ktrm t.
   Proof.
     intros. unfold toklist, compose. autorewrite with sysf_rw tea_list.
-    compose near (toklistd term KTerm t) on left. rewrite (fun_map_map (F:= list)).
+    compose near (toklistd term ktrm t) on left. rewrite (fun_map_map (F:= list)).
     repeat fequal. now ext [w a].
   Qed.
 
-  Lemma rw_toklist_KTerm_term3: forall t1 t2, toklist term KTerm (tm_app t1 t2) = toklist term KTerm t1 ++ toklist term KTerm t2.
+  Lemma rw_toklist_ktrm_term3: forall t1 t2, toklist term ktrm (tm_app t1 t2) = toklist term ktrm t1 ++ toklist term ktrm t2.
   Proof. intros. unfold toklist, compose. now autorewrite with sysf_rw tea_list. Qed.
 
-  Lemma rw_toklist_KTerm_term4: forall t, toklist term KTerm (tm_tab t) = toklist term KTerm t.
+  Lemma rw_toklist_ktrm_term4: forall t, toklist term ktrm (tm_tab t) = toklist term ktrm t.
   Proof.
     intros. unfold toklist, compose. autorewrite with sysf_rw.
-    compose near (toklistd term KTerm t) on left. rewrite (fun_map_map (F:= list)).
+    compose near (toklistd term ktrm t) on left. rewrite (fun_map_map (F:= list)).
     repeat fequal. now ext [w a].
   Qed.
 
-  Lemma rw_toklist_KTerm_term5: forall t τ, toklist term KTerm (tm_tap t τ) = toklist term KTerm t ++ toklist typ KTerm τ.
+  Lemma rw_toklist_ktrm_term5: forall t τ, toklist term ktrm (tm_tap t τ) = toklist term ktrm t ++ toklist typ ktrm τ.
   Proof. intros. unfold toklist, compose. now autorewrite with sysf_rw tea_list. Qed.
 
-End rw_toklist_KTerm_term.
+End rw_toklist_ktrm_term.
 
-#[export] Hint Rewrite @rw_toklist_KTerm_term1 @rw_toklist_KTerm_term2 @rw_toklist_KTerm_term3 @rw_toklist_KTerm_term4 @rw_toklist_KTerm_term5: sysf_rw.
+#[export] Hint Rewrite @rw_toklist_ktrm_term1 @rw_toklist_ktrm_term2 @rw_toklist_ktrm_term3 @rw_toklist_ktrm_term4 @rw_toklist_ktrm_term5: sysf_rw.
 
 (** *** Variable occurrence with context *)
 (******************************************************************************)
-Section rw_tomsetd_type.
+Section rw_tosetmd_type.
 
   Context
     (A: Type)
@@ -1498,19 +1240,19 @@ Section rw_tomsetd_type.
 
   Implicit Types (w: list K) (a: A).
 
-  Lemma rw_tomsetd_term1: forall w a a', (w, (k, a)) ∈md (tm_var a') <->  w = nil /\ k = KTerm /\ a = a'.
-    intros. unfold tomsetd, compose. autorewrite with sysf_rw.
+  Lemma rw_tosetmd_term1: forall w a a', (w, (k, a)) ∈md (tm_var a') <->  w = nil /\ k = ktrm /\ a = a'.
+    intros. unfold tosetmd, compose. autorewrite with sysf_rw.
     rewrite tosubset_list_one.
     split.
     - now inversion 1.
     - intros [? [? ?]]; now subst.
   Qed.
 
-  Lemma rw_tomsetd_term2: forall τ t w a,
+  Lemma rw_tosetmd_term2: forall τ t w a,
       (w, (k, a)) ∈md (tm_abs τ t) <->
-      (w, (k, a)) ∈md τ \/ exists w', (w', (k, a)) ∈md t /\ w = KTerm:: w'.
+      (w, (k, a)) ∈md τ \/ exists w', (w', (k, a)) ∈md t /\ w = ktrm:: w'.
   Proof.
-    intros. unfold tomsetd, compose. autorewrite with sysf_rw tea_list.
+    intros. unfold tosetmd, compose. autorewrite with sysf_rw tea_list.
     rewrite (tosubset_map_iff). split.
     - intros [hyp | hyp].
       + now left.
@@ -1522,32 +1264,32 @@ Section rw_tomsetd_type.
         exists (w', (k, a)). auto.
   Qed.
 
-  Lemma rw_tomsetd_term3: forall w a (t1 t2: term A), (w, (k, a)) ∈md tm_app t1 t2 <-> ((w, (k, a)) ∈md t1 \/ (w, (k, a)) ∈md t2).
+  Lemma rw_tosetmd_term3: forall w a (t1 t2: term A), (w, (k, a)) ∈md tm_app t1 t2 <-> ((w, (k, a)) ∈md t1 \/ (w, (k, a)) ∈md t2).
   Proof.
-    intros. unfold tomsetd, compose.
+    intros. unfold tosetmd, compose.
     now autorewrite with sysf_rw tea_list.
   Qed.
 
-  Lemma rw_tomsetd_term4: forall w a (t: term A), (w, (k, a)) ∈md (tm_tab t) <-> exists w', (w', (k, a)) ∈md t /\ w = KType:: w'.
+  Lemma rw_tosetmd_term4: forall w a (t: term A), (w, (k, a)) ∈md (tm_tab t) <-> exists w', (w', (k, a)) ∈md t /\ w = ktyp:: w'.
   Proof.
-    intros. unfold tomsetd, compose. autorewrite with sysf_rw.
+    intros. unfold tosetmd, compose. autorewrite with sysf_rw.
     rewrite (tosubset_map_iff). splits.
     - intros [[w'' [j a']] [rest1 rest2]]. cbn in *. inverts rest2. eauto.
     - intros [w' rest]. exists (w', (k, a)). now inverts rest.
   Qed.
 
-  Lemma rw_tomsetd_term5: forall w a (t: term A) (τ: typ A), (w, (k, a)) ∈md (tm_tap t τ) <-> (w, (k, a)) ∈md t \/ (w, (k, a)) ∈md τ.
+  Lemma rw_tosetmd_term5: forall w a (t: term A) (τ: typ A), (w, (k, a)) ∈md (tm_tap t τ) <-> (w, (k, a)) ∈md t \/ (w, (k, a)) ∈md τ.
   Proof.
-    intros. unfold tomsetd, compose. now autorewrite with sysf_rw tea_list.
+    intros. unfold tosetmd, compose. now autorewrite with sysf_rw tea_list.
   Qed.
 
-End rw_tomsetd_type.
+End rw_tosetmd_type.
 
-#[export] Hint Rewrite @rw_tomsetd_term1 @rw_tomsetd_term2 @rw_tomsetd_term3 @rw_tomsetd_term4 @rw_tomsetd_term5: sysf_rw.
+#[export] Hint Rewrite @rw_tosetmd_term1 @rw_tosetmd_term2 @rw_tosetmd_term3 @rw_tosetmd_term4 @rw_tosetmd_term5: sysf_rw.
 
 (** *** Variable occurrence without context *)
 (******************************************************************************)
-Section rw_tomset_type.
+Section rw_tosetm_type.
 
   Context
     (A: Type)
@@ -1555,63 +1297,63 @@ Section rw_tomset_type.
 
   Implicit Types (a: A).
 
-  Lemma rw_tomset_term1: forall a a', (k, a) ∈m tm_var a' <-> k = KTerm /\ a = a'.
-    intros. unfold tomset, compose. autorewrite with sysf_rw.
+  Lemma rw_tosetm_term1: forall a a', (k, a) ∈m tm_var a' <-> k = ktrm /\ a = a'.
+    intros. unfold tosetm, compose. autorewrite with sysf_rw.
     rewrite tosubset_list_one.
     split. inversion 1; easy. inversion 1; now subst.
   Qed.
 
-  Lemma rw_tomset_term2: forall τ t a a',
+  Lemma rw_tosetm_term2: forall τ t a a',
       (k, a) ∈m (tm_abs τ t) <-> (k, a) ∈m τ \/ (k, a) ∈m t.
   Proof.
-    intros. unfold tomset, compose. now autorewrite with sysf_rw tea_list.
+    intros. unfold tosetm, compose. now autorewrite with sysf_rw tea_list.
   Qed.
 
-  Lemma rw_tomset_term3: forall a (t1 t2: term A), (k, a) ∈m tm_app t1 t2 <-> (k, a) ∈m t1 \/ (k, a) ∈m t2.
+  Lemma rw_tosetm_term3: forall a (t1 t2: term A), (k, a) ∈m tm_app t1 t2 <-> (k, a) ∈m t1 \/ (k, a) ∈m t2.
   Proof.
-    intros. unfold tomset, compose. now autorewrite with sysf_rw tea_list.
+    intros. unfold tosetm, compose. now autorewrite with sysf_rw tea_list.
   Qed.
 
-  Lemma rw_tomset_term4: forall a (t: term A), (k, a) ∈m tm_tab t <-> (k, a) ∈m t.
+  Lemma rw_tosetm_term4: forall a (t: term A), (k, a) ∈m tm_tab t <-> (k, a) ∈m t.
   Proof.
-    intros. unfold tomset, compose. now autorewrite with sysf_rw tea_list.
+    intros. unfold tosetm, compose. now autorewrite with sysf_rw tea_list.
   Qed.
 
-  Lemma rw_tomset_term5: forall a (t: term A) (τ: typ A), (k, a) ∈m tm_tap t τ <-> (k, a) ∈m t \/ (k, a) ∈m τ.
+  Lemma rw_tosetm_term5: forall a (t: term A) (τ: typ A), (k, a) ∈m tm_tap t τ <-> (k, a) ∈m t \/ (k, a) ∈m τ.
   Proof.
-    intros. unfold tomset, compose. now autorewrite with sysf_rw tea_list.
+    intros. unfold tosetm, compose. now autorewrite with sysf_rw tea_list.
   Qed.
 
-End rw_tomset_type.
+End rw_tosetm_type.
 
-#[export] Hint Rewrite @rw_tomset_term1 @rw_tomset_term2 @rw_tomset_term3 @rw_tomset_term4 @rw_tomset_term5: sysf_rw.
+#[export] Hint Rewrite @rw_tosetm_term1 @rw_tosetm_term2 @rw_tosetm_term3 @rw_tosetm_term4 @rw_tosetm_term5: sysf_rw.
 
-(** ** <<free>> and <<freeset>> *)
+(** ** <<free>> and <<FV>> *)
 (******************************************************************************)
 
-(** *** <<free>> with <<KType>> *)
+(** *** <<free>> with <<ktyp>> *)
 (******************************************************************************)
-Section rw_free_KType_term.
+Section rw_free_ktyp_term.
 
-  Lemma rw_free_KType_term1: forall (l: LN), free term KType (tm_var l) = [].
+  Lemma rw_free_ktyp_term1: forall (l: LN), free term ktyp (tm_var l) = [].
   Proof. reflexivity. Qed.
 
-  Lemma rw_free_KType_term2: forall τ t, free term KType (tm_abs τ t) = free typ KType τ ++ free term KType t.
+  Lemma rw_free_ktyp_term2: forall τ t, free term ktyp (tm_abs τ t) = free typ ktyp τ ++ free term ktyp t.
   Proof.
     introv. unfold free. now autorewrite with sysf_rw tea_list.
   Qed.
 
-  Lemma rw_free_KType_term3: forall t1 t2, free term KType (tm_app t1 t2) = free term KType t1 ++ free term KType t2.
+  Lemma rw_free_ktyp_term3: forall t1 t2, free term ktyp (tm_app t1 t2) = free term ktyp t1 ++ free term ktyp t2.
   Proof.
     introv. unfold free. now autorewrite with sysf_rw tea_list.
   Qed.
 
-  Lemma rw_free_KType_term4: forall t, free term KType (tm_tab t) = free term KType t.
+  Lemma rw_free_ktyp_term4: forall t, free term ktyp (tm_tab t) = free term ktyp t.
   Proof.
     intros. unfold free. now autorewrite with sysf_rw.
   Qed.
 
-  Lemma rw_free_KType_term5: forall t τ, free term KType (tm_tap t τ) = free term KType t ++ free typ KType τ.
+  Lemma rw_free_ktyp_term5: forall t τ, free term ktyp (tm_tap t τ) = free term ktyp t ++ free typ ktyp τ.
   Proof.
     dup. { intros. unfold free. now autorewrite with sysf_rw tea_list. }
     intros.
@@ -1619,231 +1361,231 @@ Section rw_free_KType_term.
     unfold toklist.
     unfold compose.
     unfold toklistd.
-    unfold tomlistd.
-    unfold tomlistd_gen.
+    unfold tolistmd.
+    unfold tolistmd_gen.
     rewrite mmapdt_to_mbinddt.
     unfold compose.
   Admitted.
 
-End rw_free_KType_term.
+End rw_free_ktyp_term.
 
-#[export] Hint Rewrite rw_free_KType_term1 rw_free_KType_term2 rw_free_KType_term3 rw_free_KType_term4 rw_free_KType_term5: sysf_rw.
+#[export] Hint Rewrite rw_free_ktyp_term1 rw_free_ktyp_term2 rw_free_ktyp_term3 rw_free_ktyp_term4 rw_free_ktyp_term5: sysf_rw.
 
-(** *** <<freeset>> with <<KType>> *)
+(** *** <<FV>> with <<ktyp>> *)
 (******************************************************************************)
-Section rw_freeset_KType_term.
+Section rw_fv_ktyp_term.
 
   #[local] Open Scope set_scope.
 
-  Lemma rw_freeset_KType_term1: forall (l: LN), freeset term KType (tm_var l) [=] ∅.
+  Lemma rw_fv_ktyp_term1: forall (l: LN), FV term ktyp (tm_var l) [=] ∅.
   Proof. reflexivity. Qed.
 
-  Lemma rw_freeset_KType_term2: forall τ t, freeset term KType (tm_abs τ t) [=] freeset typ KType τ ∪ freeset term KType t.
+  Lemma rw_fv_ktyp_term2: forall τ t, FV term ktyp (tm_abs τ t) [=] FV typ ktyp τ ∪ FV term ktyp t.
   Proof.
-    introv. unfold freeset. now autorewrite with sysf_rw tea_rw_atoms.
+    introv. unfold FV. now autorewrite with sysf_rw tea_rw_atoms.
   Qed.
 
-  Lemma rw_freeset_KType_term3: forall t1 t2, freeset term KType (tm_app t1 t2) [=] freeset term KType t1 ∪ freeset term KType t2.
+  Lemma rw_fv_ktyp_term3: forall t1 t2, FV term ktyp (tm_app t1 t2) [=] FV term ktyp t1 ∪ FV term ktyp t2.
   Proof.
-    introv. unfold freeset. now autorewrite with sysf_rw tea_rw_atoms.
+    introv. unfold FV. now autorewrite with sysf_rw tea_rw_atoms.
   Qed.
 
-  Lemma rw_freeset_KType_term4: forall t, freeset term KType (tm_tab t) [=] freeset term KType t.
+  Lemma rw_fv_ktyp_term4: forall t, FV term ktyp (tm_tab t) [=] FV term ktyp t.
   Proof.
-    intros. unfold freeset. now autorewrite with sysf_rw.
+    intros. unfold FV. now autorewrite with sysf_rw.
   Qed.
 
-  Lemma rw_freeset_KType_term5: forall t τ, freeset term KType (tm_tap t τ) [=] freeset term KType t ∪ freeset typ KType τ.
+  Lemma rw_fv_ktyp_term5: forall t τ, FV term ktyp (tm_tap t τ) [=] FV term ktyp t ∪ FV typ ktyp τ.
   Proof.
-    intros. unfold freeset. now autorewrite with sysf_rw tea_rw_atoms.
+    intros. unfold FV. now autorewrite with sysf_rw tea_rw_atoms.
   Qed.
 
-End rw_freeset_KType_term.
+End rw_fv_ktyp_term.
 
-#[export] Hint Rewrite rw_freeset_KType_term1 rw_freeset_KType_term2 rw_freeset_KType_term3 rw_freeset_KType_term4 rw_freeset_KType_term5: sysf_rw.
+#[export] Hint Rewrite rw_fv_ktyp_term1 rw_fv_ktyp_term2 rw_fv_ktyp_term3 rw_fv_ktyp_term4 rw_fv_ktyp_term5: sysf_rw.
 
-(** *** <<free>> with <<KTerm>> *)
+(** *** <<free>> with <<ktrm>> *)
 (******************************************************************************)
-Section rw_free_KTerm_term.
+Section rw_free_ktrm_term.
 
-  Lemma rw_free_KTerm_term11: forall (x: atom), free term KTerm (tm_var (Fr x)) = [ x ].
+  Lemma rw_free_ktrm_term11: forall (x: atom), free term ktrm (tm_var (Fr x)) = [ x ].
   Proof. reflexivity. Qed.
 
-  Lemma rw_free_KTerm_term12: forall (n: nat), free term KTerm (tm_var (Bd n)) = [ ].
+  Lemma rw_free_ktrm_term12: forall (n: nat), free term ktrm (tm_var (Bd n)) = [ ].
   Proof. reflexivity. Qed.
 
-  Lemma rw_free_KTerm_term2: forall τ t, free term KTerm (tm_abs τ t) = free typ KTerm τ ++ free term KTerm t.
+  Lemma rw_free_ktrm_term2: forall τ t, free term ktrm (tm_abs τ t) = free typ ktrm τ ++ free term ktrm t.
   Proof.
     introv. unfold free. now autorewrite with sysf_rw tea_list.
   Qed.
 
-  Lemma rw_free_KTerm_term3: forall t1 t2, free term KTerm (tm_app t1 t2) = free term KTerm t1 ++ free term KTerm t2.
+  Lemma rw_free_ktrm_term3: forall t1 t2, free term ktrm (tm_app t1 t2) = free term ktrm t1 ++ free term ktrm t2.
   Proof.
     introv. unfold free. now autorewrite with sysf_rw tea_list.
   Qed.
 
-  Lemma rw_free_KTerm_term4: forall t, free term KTerm (tm_tab t) = free term KTerm t.
+  Lemma rw_free_ktrm_term4: forall t, free term ktrm (tm_tab t) = free term ktrm t.
   Proof.
     intros. unfold free. now autorewrite with sysf_rw.
   Qed.
 
-  Lemma rw_free_KTerm_term5: forall t τ, free term KTerm (tm_tap t τ) = free term KTerm t ++ free typ KTerm τ.
+  Lemma rw_free_ktrm_term5: forall t τ, free term ktrm (tm_tap t τ) = free term ktrm t ++ free typ ktrm τ.
   Proof.
     intros. unfold free. now autorewrite with sysf_rw tea_list.
   Qed.
 
-End rw_free_KTerm_term.
+End rw_free_ktrm_term.
 
-#[export] Hint Rewrite rw_free_KTerm_term11 rw_free_KTerm_term12 rw_free_KTerm_term2 rw_free_KTerm_term3 rw_free_KTerm_term4 rw_free_KTerm_term5: sysf_rw.
+#[export] Hint Rewrite rw_free_ktrm_term11 rw_free_ktrm_term12 rw_free_ktrm_term2 rw_free_ktrm_term3 rw_free_ktrm_term4 rw_free_ktrm_term5: sysf_rw.
 
-(** *** <<freeset>> with <<KTerm>> *)
+(** *** <<FV>> with <<ktrm>> *)
 (******************************************************************************)
-Section rw_freeset_KTerm_term.
+Section rw_fv_ktrm_term.
 
   #[local] Open Scope set_scope.
 
-  Lemma rw_freeset_KTerm_term11: forall (x: atom), freeset term KTerm (tm_var (Fr x)) [=] {{ x }}.
+  Lemma rw_fv_ktrm_term11: forall (x: atom), FV term ktrm (tm_var (Fr x)) [=] {{ x }}.
   Proof.
-    introv. unfold freeset. now autorewrite with sysf_rw.
+    introv. unfold FV. now autorewrite with sysf_rw.
   Qed.
 
-  Lemma rw_freeset_KTerm_term12: forall (n: nat), freeset term KTerm (tm_var (Bd n)) [=] ∅.
+  Lemma rw_fv_ktrm_term12: forall (n: nat), FV term ktrm (tm_var (Bd n)) [=] ∅.
   Proof. reflexivity. Qed.
 
-  Lemma rw_freeset_KTerm_term2: forall τ t, freeset term KTerm (tm_abs τ t) [=] freeset typ KTerm τ ∪ freeset term KTerm t.
+  Lemma rw_fv_ktrm_term2: forall τ t, FV term ktrm (tm_abs τ t) [=] FV typ ktrm τ ∪ FV term ktrm t.
   Proof.
-    introv. unfold freeset. now autorewrite with sysf_rw tea_rw_atoms.
+    introv. unfold FV. now autorewrite with sysf_rw tea_rw_atoms.
   Qed.
 
-  Lemma rw_freeset_KTerm_term3: forall t1 t2, freeset term KTerm (tm_app t1 t2) [=] freeset term KTerm t1 ∪ freeset term KTerm t2.
+  Lemma rw_fv_ktrm_term3: forall t1 t2, FV term ktrm (tm_app t1 t2) [=] FV term ktrm t1 ∪ FV term ktrm t2.
   Proof.
-    introv. unfold freeset. now autorewrite with sysf_rw tea_rw_atoms.
+    introv. unfold FV. now autorewrite with sysf_rw tea_rw_atoms.
   Qed.
 
-  Lemma rw_freeset_KTerm_term4: forall t, freeset term KTerm (tm_tab t) [=] freeset term KTerm t.
+  Lemma rw_fv_ktrm_term4: forall t, FV term ktrm (tm_tab t) [=] FV term ktrm t.
   Proof.
-    intros. unfold freeset. now autorewrite with sysf_rw.
+    intros. unfold FV. now autorewrite with sysf_rw.
   Qed.
 
-  Lemma rw_freeset_KTerm_term5: forall t τ, freeset term KTerm (tm_tap t τ) [=] freeset term KTerm t ∪ freeset typ KTerm τ.
+  Lemma rw_fv_ktrm_term5: forall t τ, FV term ktrm (tm_tap t τ) [=] FV term ktrm t ∪ FV typ ktrm τ.
   Proof.
-    intros. unfold freeset. now autorewrite with sysf_rw tea_rw_atoms.
+    intros. unfold FV. now autorewrite with sysf_rw tea_rw_atoms.
   Qed.
 
-End rw_freeset_KTerm_term.
+End rw_fv_ktrm_term.
 
-#[export] Hint Rewrite rw_freeset_KTerm_term11 rw_freeset_KTerm_term12 rw_freeset_KTerm_term2 rw_freeset_KTerm_term3 rw_freeset_KTerm_term4 rw_freeset_KTerm_term5: sysf_rw.
+#[export] Hint Rewrite rw_fv_ktrm_term11 rw_fv_ktrm_term12 rw_fv_ktrm_term2 rw_fv_ktrm_term3 rw_fv_ktrm_term4 rw_fv_ktrm_term5: sysf_rw.
 
 (** ** Locally nameless operations *)
 (******************************************************************************)
 
-(** *** <<subst>> with <<KType>> *)
+(** *** <<subst>> with <<ktyp>> *)
 (******************************************************************************)
-Section rw_subst_KType_term.
+Section rw_subst_ktyp_term.
 
   Context
     (x: atom)
     (u: typ LN).
 
-  Lemma rw_subst_KType_term1: forall l, subst term KType x u (tm_var l) = tm_var l.
+  Lemma rw_subst_ktyp_term1: forall l, subst term ktyp x u (tm_var l) = tm_var l.
   Proof. reflexivity. Qed.
 
-  Lemma rw_subst_KType_term2: forall τ t, subst term KType x u (tm_abs τ t) = tm_abs (subst typ KType x u τ) (subst term KType x u t).
+  Lemma rw_subst_ktyp_term2: forall τ t, subst term ktyp x u (tm_abs τ t) = tm_abs (subst typ ktyp x u τ) (subst term ktyp x u t).
   Proof.
     introv. unfold subst. now autorewrite with sysf_rw.
   Qed.
 
-  Lemma rw_subst_KType_term3: forall t1 t2, subst term KType x u (tm_app t1 t2) = tm_app (subst term KType x u t1) (subst term KType x u t2).
+  Lemma rw_subst_ktyp_term3: forall t1 t2, subst term ktyp x u (tm_app t1 t2) = tm_app (subst term ktyp x u t1) (subst term ktyp x u t2).
   Proof. reflexivity. Qed.
 
-  Lemma rw_subst_KType_term4: forall t, subst term KType x u (tm_tab t) = tm_tab (subst term KType x u t).
+  Lemma rw_subst_ktyp_term4: forall t, subst term ktyp x u (tm_tab t) = tm_tab (subst term ktyp x u t).
   Proof.
     introv. unfold subst. now autorewrite with sysf_rw.
   Qed.
 
-  Lemma rw_subst_KType_term5: forall t τ, subst term KType x u (tm_tap t τ) = tm_tap (subst term KType x u t) (subst typ KType x u τ).
+  Lemma rw_subst_ktyp_term5: forall t τ, subst term ktyp x u (tm_tap t τ) = tm_tap (subst term ktyp x u t) (subst typ ktyp x u τ).
   Proof. reflexivity. Qed.
 
-End rw_subst_KType_term.
+End rw_subst_ktyp_term.
 
-#[export] Hint Rewrite @rw_subst_KType_term1 @rw_subst_KType_term2 @rw_subst_KType_term3 @rw_subst_KType_term4 @rw_subst_KType_term5: sysf_rw.
+#[export] Hint Rewrite @rw_subst_ktyp_term1 @rw_subst_ktyp_term2 @rw_subst_ktyp_term3 @rw_subst_ktyp_term4 @rw_subst_ktyp_term5: sysf_rw.
 
-(** *** <<subst>> with <<KTerm>> *)
+(** *** <<subst>> with <<ktrm>> *)
 (******************************************************************************)
-Section rw_subst_KTerm_term.
+Section rw_subst_ktrm_term.
 
   Context
     (x: atom)
     (u: term LN).
 
-  Lemma rw_subst_KTerm_term11: subst term KTerm x u (tm_var (Fr x)) = u.
+  Lemma rw_subst_ktrm_term11: subst term ktrm x u (tm_var (Fr x)) = u.
   Proof. unfold subst. autorewrite with sysf_rw. cbn. compare values x and x. Qed.
 
-  Lemma rw_subst_KTerm_term12: forall (y: atom), x <> y -> subst term KTerm x u (tm_var (Fr y)) = tm_var (Fr y).
+  Lemma rw_subst_ktrm_term12: forall (y: atom), x <> y -> subst term ktrm x u (tm_var (Fr y)) = tm_var (Fr y).
   Proof. intros. unfold subst. autorewrite with sysf_rw. cbn. compare values x and y. Qed.
 
-  Lemma rw_subst_KTerm_term13: forall (n: nat), subst term KTerm x u (tm_var (Bd n)) = tm_var (Bd n).
+  Lemma rw_subst_ktrm_term13: forall (n: nat), subst term ktrm x u (tm_var (Bd n)) = tm_var (Bd n).
   Proof. reflexivity. Qed.
 
-  Lemma rw_subst_KTerm_term2: forall τ t, subst term KTerm x u (tm_abs τ t) = tm_abs (subst typ KTerm x u τ) (subst term KTerm x u t).
+  Lemma rw_subst_ktrm_term2: forall τ t, subst term ktrm x u (tm_abs τ t) = tm_abs (subst typ ktrm x u τ) (subst term ktrm x u t).
   Proof.
     introv. unfold subst. now autorewrite with sysf_rw.
   Qed.
 
-  Lemma rw_subst_KTerm_term3: forall t1 t2, subst term KTerm x u (tm_app t1 t2) = tm_app (subst term KTerm x u t1) (subst term KTerm x u t2).
+  Lemma rw_subst_ktrm_term3: forall t1 t2, subst term ktrm x u (tm_app t1 t2) = tm_app (subst term ktrm x u t1) (subst term ktrm x u t2).
   Proof. reflexivity. Qed.
 
-  Lemma rw_subst_KTerm_term4: forall t, subst term KTerm x u (tm_tab t) = tm_tab (subst term KTerm x u t).
+  Lemma rw_subst_ktrm_term4: forall t, subst term ktrm x u (tm_tab t) = tm_tab (subst term ktrm x u t).
   Proof.
     introv. unfold subst. now autorewrite with sysf_rw.
   Qed.
 
-  Lemma rw_subst_KTerm_term5: forall t τ, subst term KTerm x u (tm_tap t τ) = tm_tap (subst term KTerm x u t) (subst typ KTerm x u τ).
+  Lemma rw_subst_ktrm_term5: forall t τ, subst term ktrm x u (tm_tap t τ) = tm_tap (subst term ktrm x u t) (subst typ ktrm x u τ).
   Proof. reflexivity. Qed.
 
-End rw_subst_KTerm_term.
+End rw_subst_ktrm_term.
 
-#[export] Hint Rewrite @rw_subst_KTerm_term11 @rw_subst_KTerm_term12 @rw_subst_KTerm_term13 @rw_subst_KTerm_term2 @rw_subst_KTerm_term3 @rw_subst_KTerm_term4 @rw_subst_KTerm_term5: sysf_rw.
+#[export] Hint Rewrite @rw_subst_ktrm_term11 @rw_subst_ktrm_term12 @rw_subst_ktrm_term13 @rw_subst_ktrm_term2 @rw_subst_ktrm_term3 @rw_subst_ktrm_term4 @rw_subst_ktrm_term5: sysf_rw.
 
 #[local] Open Scope nat_scope.
 
-(** *** <<locally_closed>> with <<KType>> *)
+(** *** <<locally_closed>> with <<ktyp>> *)
 (******************************************************************************)
-Section rw_lc_KType_term.
+Section rw_lc_ktyp_term.
 
-  Lemma rw_lc_KType_term1: forall l, locally_closed term KType (tm_var l).
+  Lemma rw_lc_ktyp_term1: forall l, locally_closed term ktyp (tm_var l).
   Proof.
     intros. unfold locally_closed, locally_closed_gap.
     introv. autorewrite with sysf_rw. introv [? [? ?]]; now subst.
   Qed.
 
-  Lemma rw_lc_KType_term2: forall (τ: typ LN) (t: term LN), locally_closed term KType (tm_abs τ t) <-> locally_closed typ KType τ /\ locally_closed term KType t.
+  Lemma rw_lc_ktyp_term2: forall (τ: typ LN) (t: term LN), locally_closed term ktyp (tm_abs τ t) <-> locally_closed typ ktyp τ /\ locally_closed term ktyp t.
   Proof.
     intros. unfold locally_closed, locally_closed_gap.
-    setoid_rewrite rw_tomsetd_term2. split.
+    setoid_rewrite rw_tosetmd_term2. split.
     - introv hyp. split.
       + intros. apply (hyp w l). now left.
-      + intros. apply (hyp (KTerm:: w) l). right. eauto.
+      + intros. apply (hyp (ktrm:: w) l). right. eauto.
     - introv [hyp1 hyp2]. introv [hyp | hyp].
       + auto.
       + inverts hyp. inverts H. cbn. now apply hyp2.
   Qed.
 
-  Lemma rw_lc_KType_term3: forall (t1 t2: term LN), locally_closed term KType (tm_app t1 t2) <-> locally_closed term KType t1 /\ locally_closed term KType t2.
+  Lemma rw_lc_ktyp_term3: forall (t1 t2: term LN), locally_closed term ktyp (tm_app t1 t2) <-> locally_closed term ktyp t1 /\ locally_closed term ktyp t2.
   Proof.
     intros. unfold locally_closed, locally_closed_gap.
-    setoid_rewrite rw_tomsetd_term3. firstorder.
+    setoid_rewrite rw_tosetmd_term3. firstorder.
   Qed.
 
   #[local] Open Scope nat_scope.
 
-  Lemma rw_lc_KType_term4: forall t, locally_closed term KType (tm_tab t) <-> locally_closed_gap term KType 1 t.
+  Lemma rw_lc_ktyp_term4: forall t, locally_closed term ktyp (tm_tab t) <-> locally_closed_gap term ktyp 1 t.
   Proof.
     intros. unfold locally_closed, locally_closed_gap.
-    setoid_rewrite rw_tomsetd_term4. split.
+    setoid_rewrite rw_tosetmd_term4. split.
     - intros hyp w l Hin.
-      specialize (hyp (KType:: w) l). cbn in *.
-      assert (rw: S (countk (@KType: K) w + 0) = (countk KType w + 1)) by lia.
+      specialize (hyp (ktyp:: w) l). cbn in *.
+      assert (rw: S (countk (@ktyp: K) w + 0) = (countk ktyp w + 1)) by lia.
       rewrite <- rw. apply hyp. eauto.
     - intros hyp w l [w' [H1 H2]]. subst.
       specialize (hyp w' l H1). cbn in *. destruct l.
@@ -1851,94 +1593,94 @@ Section rw_lc_KType_term.
       + lia.
   Qed.
 
-  Lemma rw_lc_KType_term5: forall t τ, locally_closed term KType (tm_tap t τ) <-> locally_closed term KType t /\ locally_closed typ KType τ.
+  Lemma rw_lc_ktyp_term5: forall t τ, locally_closed term ktyp (tm_tap t τ) <-> locally_closed term ktyp t /\ locally_closed typ ktyp τ.
   Proof.
     intros. unfold locally_closed, locally_closed_gap.
-    setoid_rewrite rw_tomsetd_term5. split.
+    setoid_rewrite rw_tosetmd_term5. split.
     - introv hyp1. split.
       + introv hyp2. apply hyp1. now left.
       + introv hyp2. apply hyp1. now right.
     - introv [hyp1 hyp2] [hyp | hyp]; auto.
   Qed.
 
-End rw_lc_KType_term.
+End rw_lc_ktyp_term.
 
-#[export] Hint Rewrite @rw_lc_KType_term1 @rw_lc_KType_term2 @rw_lc_KType_term3 @rw_lc_KType_term4 @rw_lc_KType_term5: sysf_rw.
+#[export] Hint Rewrite @rw_lc_ktyp_term1 @rw_lc_ktyp_term2 @rw_lc_ktyp_term3 @rw_lc_ktyp_term4 @rw_lc_ktyp_term5: sysf_rw.
 
-(** *** <<locally_closed>> with <<KTerm>> *)
+(** *** <<locally_closed>> with <<ktrm>> *)
 (******************************************************************************)
-Section rw_lc_KTerm_term.
+Section rw_lc_ktrm_term.
 
-  Lemma rw_lc_KTerm_term11: forall x, locally_closed term KTerm (tm_var (Fr x)).
+  Lemma rw_lc_ktrm_term11: forall x, locally_closed term ktrm (tm_var (Fr x)).
   Proof.
     intros. unfold locally_closed, locally_closed_gap.
     introv. autorewrite with sysf_rw. introv [? [? ?]]; now subst.
   Qed.
 
-  Lemma rw_lc_KTerm_term12: forall n, locally_closed term KTerm (tm_var (Bd n)) <-> False.
+  Lemma rw_lc_ktrm_term12: forall n, locally_closed term ktrm (tm_var (Bd n)) <-> False.
   Proof.
     intros. unfold locally_closed, locally_closed_gap.
     split; [ |intuition]. introv hyp. cbn in hyp.
     specialize (hyp [] (Bd n) ltac:(auto)). cbn in hyp. lia.
   Qed.
 
-  Lemma rw_lc_KTerm_term2: forall (τ: typ LN) (t: term LN), locally_closed term KTerm (tm_abs τ t) <-> locally_closed typ KTerm τ /\ locally_closed_gap term KTerm 1 t.
+  Lemma rw_lc_ktrm_term2: forall (τ: typ LN) (t: term LN), locally_closed term ktrm (tm_abs τ t) <-> locally_closed typ ktrm τ /\ locally_closed_gap term ktrm 1 t.
   Proof.
     intros. unfold locally_closed, locally_closed_gap.
-    setoid_rewrite rw_tomsetd_term2. split.
+    setoid_rewrite rw_tosetmd_term2. split.
     - introv hyp. split.
       + intros. apply (hyp w l). now left.
-      + intros. specialize (hyp (KTerm:: w) l). cbn in *.
-      assert (rw: S (countk (@KTerm: K) w + 0) = (countk KTerm w + 1)) by lia.
+      + intros. specialize (hyp (ktrm:: w) l). cbn in *.
+      assert (rw: S (countk (@ktrm: K) w + 0) = (countk ktrm w + 1)) by lia.
       rewrite <- rw. apply hyp. eauto.
     - introv [hyp1 hyp2]. introv [hyp | hyp].
       + auto.
       + destruct hyp as [w' [hyp' hyp'']]. subst. cbn in *.
-      assert (rw: S (countk (@KTerm: K) w' + 0) = (countk KTerm w' + 1)) by lia.
+      assert (rw: S (countk (@ktrm: K) w' + 0) = (countk ktrm w' + 1)) by lia.
       rewrite rw. apply hyp2. auto.
   Qed.
 
-  Lemma rw_lc_KTerm_term3: forall (t1 t2: term LN), locally_closed term KTerm (tm_app t1 t2) <-> locally_closed term KTerm t1 /\ locally_closed term KTerm t2.
+  Lemma rw_lc_ktrm_term3: forall (t1 t2: term LN), locally_closed term ktrm (tm_app t1 t2) <-> locally_closed term ktrm t1 /\ locally_closed term ktrm t2.
   Proof.
     intros. unfold locally_closed, locally_closed_gap.
-    setoid_rewrite rw_tomsetd_term3. firstorder.
+    setoid_rewrite rw_tosetmd_term3. firstorder.
   Qed.
 
   #[local] Open Scope nat_scope.
 
-  Lemma rw_lc_KTerm_term4: forall t, locally_closed term KTerm (tm_tab t) <-> locally_closed term KTerm t.
+  Lemma rw_lc_ktrm_term4: forall t, locally_closed term ktrm (tm_tab t) <-> locally_closed term ktrm t.
   Proof.
     intros. unfold locally_closed, locally_closed_gap.
-    setoid_rewrite rw_tomsetd_term4. split.
-    - intros hyp w l Hin. specialize (hyp (KType:: w) l).
+    setoid_rewrite rw_tosetmd_term4. split.
+    - intros hyp w l Hin. specialize (hyp (ktyp:: w) l).
       apply hyp. eauto.
     - intros hyp w l [w' [rest1 rest2]]. subst.
       cbn. apply hyp; auto.
   Qed.
 
-  Lemma rw_lc_KTerm_term5: forall t τ, locally_closed term KTerm (tm_tap t τ) <-> locally_closed term KTerm t /\ locally_closed typ KTerm τ.
+  Lemma rw_lc_ktrm_term5: forall t τ, locally_closed term ktrm (tm_tap t τ) <-> locally_closed term ktrm t /\ locally_closed typ ktrm τ.
   Proof.
     intros. unfold locally_closed, locally_closed_gap.
-    setoid_rewrite rw_tomsetd_term5. split.
+    setoid_rewrite rw_tosetmd_term5. split.
     - introv hyp1. split.
       + introv hyp2. apply hyp1. now left.
       + introv hyp2. apply hyp1. now right.
     - introv [hyp1 hyp2] [hyp | hyp]; auto.
   Qed.
 
-End rw_lc_KTerm_term.
+End rw_lc_ktrm_term.
 
-#[export] Hint Rewrite @rw_lc_KTerm_term11 @rw_lc_KTerm_term12 @rw_lc_KTerm_term2 @rw_lc_KTerm_term3 @rw_lc_KTerm_term4 @rw_lc_KTerm_term5: sysf_rw.
+#[export] Hint Rewrite @rw_lc_ktrm_term11 @rw_lc_ktrm_term12 @rw_lc_ktrm_term2 @rw_lc_ktrm_term3 @rw_lc_ktrm_term4 @rw_lc_ktrm_term5: sysf_rw.
 
 (** * Rewriting principles for <<ok_term>> *)
 (******************************************************************************)
 Lemma ok_term_abs: forall Δ Γ τ t,
     ok_term Δ Γ (tm_abs τ t) <->
     ok_type Δ τ /\
-    scoped term KTerm t (AssocList.domset Γ) /\
-    scoped term KType t (AssocList.domset Δ) /\
-    locally_closed term KType t /\
-    locally_closed_gap term KTerm 1 t.
+    scoped term ktrm t (AssocList.domset Γ) /\
+    scoped term ktyp t (AssocList.domset Δ) /\
+    locally_closed term ktyp t /\
+    locally_closed_gap term ktrm 1 t.
 Proof.
   intros. unfold ok_type, ok_term.
   unfold scoped.
