Tealeaves/Simplification/MBinddt.v
@@ -1,0 +1,95 @@
+From Tealeaves Require Export
+  Simplification.Support
+  Simplification.Binddt
+  Theory.Multisorted.DecoratedTraversableMonad.
+
+Import
+  List.ListNotations
+  Product.Notations
+  Monoid.Notations
+  ContainerFunctor.Notations
+  Subset.Notations.
+
+(** * Rewriting with binddt *)
+(******************************************************************************)
+Module ToBinddt.
+
+  Ltac rewrite_core_ops_to_binddt :=
+    match goal with
+    | |- context[mmap ?f ?t] =>
+        ltac_trace "mmap_to_mbinddt";
+        progress (rewrite mmap_to_mbinddt)
+    (* mapd/bind/traverse *)
+    | |- context[mbind ?f ?t] =>
+        ltac_trace "mbind_to_mbinddt";
+        progress (rewrite mbind_to_mbinddt)
+    | |- context[mmapd ?f ?t] =>
+        ltac_trace "mmapd_to_mbinddt";
+        progress (rewrite mmapd_to_mbinddt)
+    (* mmapdt/bindd/bindt *)
+    | |- context[mmapdt ?f ?t] =>
+        ltac_trace "mmapdt_to_mbinddt";
+        progress (rewrite mmapdt_to_mbinddt)
+    | |- context[mbindd ?f ?t] =>
+        ltac_trace "mbindd_to_mbinddt";
+        progress (rewrite mbindd_to_mbinddt)
+    | |- context[bindt ?f ?t] =>
+        ltac_trace "bindt_to_mbinddt";
+        progress (rewrite mbindt_to_mbinddt)
+    end.
+
+  (*
+  Ltac rewrite_derived_ops_to_binddt T :=
+    match goal with
+    (* tolist *)
+    | |- context[tolist (F := T) ?t] =>
+        ltac_trace "tolist_to_binddt";
+        rewrite (tolist_to_binddt (T := T))
+    (* elements *)
+    | |- context[element_of (F := T) ?x ?t] =>
+        ltac_trace "element_of_to_binddt";
+        rewrite (element_of_to_binddt (T := T))
+    | |- context[element_ctx_of (T := T) (?n, ?l) ?t] =>
+        ltac_trace "element_ctx_of_to_binddt";
+        rewrite (element_ctx_of_to_binddt (T := T))
+    (* tosubset *)
+    | |- context[tosubset (F := T) ?t] =>
+        ltac_trace "tosubset_to_binddt";
+        rewrite (tosubset_to_binddt (T := T))
+    | |- context[toctxset (F := T) ?t] =>
+        ltac_trace "toctxset_to_binddt";
+        rewrite (toctxset_to_binddt (T := T))
+    (* foldMap *)
+    | |- context[foldMap (T := T) ?t] =>
+        ltac_trace "foldMap_to_binddt";
+        rewrite foldMap_to_traverse1, traverse_to_binddt
+    | |- context[foldMapd (T := T) ?t] =>
+        ltac_trace "foldMap_to_binddt";
+        rewrite (foldMapd_to_mapdt1 (T := T)),
+          (mapdt_to_binddt (T := T))
+    (* quantifiers *)
+    | |- context[Forall_ctx (T := T)  ?P] =>
+        ltac_trace "Forall_to_foldMapd";
+        unfold Forall_ctx
+    end.
+    *)
+
+End ToBinddt.
+
+(*|
+If we find some <<binddt f t>>, simplify it with cbn.
+|*)
+Ltac cbn_mbinddt :=
+  match goal with
+  | |- context[mbinddt (W := ?W) (T := ?T)
+                (H := ?H) (H0 := ?H0) (H1 := ?H1)
+                ?U ?F ?f ?t] =>
+      let e := constr:(mbinddt (W := W) (T := T) U F
+                         (H := H) (H0 := H0) (H1 := H1)
+                         f t) in
+      cbn_subterm e
+      (*
+      let e' := eval cbn in e in
+        progress (change e with e')
+       *)
+  end.
